use variables instead of parameters

src/fol.lean
@@ -134,7 +134,7 @@ end
 
 /- 
   Note: we only work in the bottom universe. If we don't, then when we define the realization of
-  formulae in a structure S, we want to send preformula n to 
+  formulae in a Structure L S, we want to send preformula n to 
   S → (S → ... → (S → Prop)...)
   with n occurrences of S. If S : Type u, then this type lives in `Type u` for n ≥ 1 and in Type 0 for n = 0, which is super inconvenient/impossible to work with
 -/
@@ -143,10 +143,10 @@ structure Language : Type (u+1) :=
 
 def Language.constants (L : Language) := L.functions 0
 section
-parameter (L : Language.{u})
+variable (L : Language.{u})
 
-/- preterm l is a partially applied term. if applied to n terms, it becomes a term.
-* Every element of preterm 0 is well typed. 
+/- preterm L l is a partially applied term. if applied to n terms, it becomes a term.
+* Every element of preterm L 0 is a well-formed term. 
 * We use this encoding to avoid mutual or nested inductive types, since those are not too convenient to work with in Lean. -/
 inductive preterm : ℕ → Type u
 | var {} : ∀ (k : ℕ), preterm 0
@@ -154,36 +154,36 @@ inductive preterm : ℕ → Type u
 | app : ∀ {l : ℕ} (t : preterm (l + 1)) (s : preterm 0), preterm l
 export preterm
 
-@[reducible] def term := preterm 0
+@[reducible] def term := preterm L 0
 
-parameter {L}
+variable {L}
 prefix `&`:max := _root_.fol.preterm.var
 
-@[simp] def apps : ∀{l}, preterm l → dvector term l → term
+@[simp] def apps : ∀{l}, preterm L l → dvector (term L) l → term L
 | _ t []       := t
 | _ t (t'::ts) := apps (app t t') ts
 
-@[simp] lemma apps_zero (t : term) (ts : dvector term 0) : apps t ts = t :=
+@[simp] lemma apps_zero (t : term L) (ts : dvector (term L) 0) : apps t ts = t :=
 by cases ts; refl
 
-def term_of_function {l} (f : L.functions l) : arity term term l :=
+def term_of_function {l} (f : L.functions l) : arity (term L) (term L) l :=
 arity.of_dvector_map $ apps (func f)
 
 /- lift_term_at _ t n m raises variables in t which are at least m by n -/
-@[simp] def lift_term_at : ∀ {l}, preterm l → ℕ → ℕ → preterm l
+@[simp] def lift_term_at : ∀ {l}, preterm L l → ℕ → ℕ → preterm L l
 | _ &k          n m := if m ≤ k then &(k+n) else &k
 | _ (func f)    n m := func f
 | _ (app t₁ t₂) n m := app (lift_term_at t₁ n m) (lift_term_at t₂ n m)
 
 notation t ` ↑' `:90 n ` # `:90 m:90 := _root_.fol.lift_term_at t n m -- input ↑ with \u or \upa
 
-@[reducible] def lift_term {l} (t : preterm l) (n : ℕ) : preterm l := t ↑' n # 0
+@[reducible] def lift_term {l} (t : preterm L l) (n : ℕ) : preterm L l := t ↑' n # 0
 infix ` ↑ `:100 := _root_.fol.lift_term -- input ↑' with \u or \upa
-@[reducible, simp] def lift_term1 {l} (t : preterm l) : preterm l := t ↑ 1
+@[reducible, simp] def lift_term1 {l} (t : preterm L l) : preterm L l := t ↑ 1
 
-@[simp] lemma lift_term_def {l} (t : preterm l) (n : ℕ) : t ↑' n # 0 = t ↑ n := by refl
+@[simp] lemma lift_term_def {l} (t : preterm L l) (n : ℕ) : t ↑' n # 0 = t ↑ n := by refl
 
-lemma lift_term_at_inj : ∀ {l} {t t' : preterm l} {n m : ℕ}, t ↑' n # m = t' ↑' n # m → t = t'
+lemma lift_term_at_inj : ∀ {l} {t t' : preterm L l} {n m : ℕ}, t ↑' n # m = t' ↑' n # m → t = t'
 | _ &k &k' n m h := 
   by by_cases h₁ : m ≤ k; by_cases h₂ : m ≤ k'; simp [h₁, h₂] at h;
      congr;[assumption, skip, skip, assumption]; exfalso; try {apply h₁}; 
@@ -198,15 +198,15 @@ lemma lift_term_at_inj : ∀ {l} {t t' : preterm l} {n m : ℕ}, t ↑' n # m = 
 | _ (app t₁ t₂) (app t₁' t₂') n m h := 
   begin injection h, congr; apply lift_term_at_inj; assumption end
 
-@[simp] lemma lift_term_at_zero : ∀ {l} (t : preterm l) (m : ℕ), t ↑' 0 # m = t
+@[simp] lemma lift_term_at_zero : ∀ {l} (t : preterm L l) (m : ℕ), t ↑' 0 # m = t
 | _ &k          m := by simp
 | _ (func f)    m := by refl
 | _ (app t₁ t₂) m := by dsimp; congr; apply lift_term_at_zero
 
-@[simp] lemma lift_term_zero {l} (t : preterm l) : t ↑ 0 = t := lift_term_at_zero t 0
+@[simp] lemma lift_term_zero {l} (t : preterm L l) : t ↑ 0 = t := lift_term_at_zero t 0
 
 /- the following lemmas simplify iterated lifts, depending on the size of m' -/
-lemma lift_term_at2_small : ∀ {l} (t : preterm l) (n n') {m m'}, m' ≤ m → 
+lemma lift_term_at2_small : ∀ {l} (t : preterm L l) (n n') {m m'}, m' ≤ m → 
   (t ↑' n # m) ↑' n' # m' = (t ↑' n' # m') ↑' n # (m + n')
 | _ &k          n n' m m' H := 
   begin 
@@ -222,7 +222,7 @@ lemma lift_term_at2_small : ∀ {l} (t : preterm l) (n n') {m m'}, m' ≤ m →
 | _ (app t₁ t₂) n n' m m' H := 
   begin dsimp; congr1; apply lift_term_at2_small; assumption end
 
-lemma lift_term_at2_medium : ∀ {l} (t : preterm l) {n} (n') {m m'}, m ≤ m' → m' ≤ m+n → 
+lemma lift_term_at2_medium : ∀ {l} (t : preterm L l) {n} (n') {m m'}, m ≤ m' → m' ≤ m+n → 
   (t ↑' n # m) ↑' n' # m' = t ↑' (n+n') # m
 | _ &k          n n' m m' H₁ H₂ := 
   begin 
@@ -234,54 +234,54 @@ lemma lift_term_at2_medium : ∀ {l} (t : preterm l) {n} (n') {m m'}, m ≤ m' �
 | _ (app t₁ t₂) n n' m m' H₁ H₂ := 
   begin dsimp; congr1; apply lift_term_at2_medium; assumption end
 
-lemma lift_term2_medium {l} (t : preterm l) {n} (n') {m'} (h : m' ≤ n) :
+lemma lift_term2_medium {l} (t : preterm L l) {n} (n') {m'} (h : m' ≤ n) :
   (t ↑ n) ↑' n' # m' = t ↑ (n+n') :=
 lift_term_at2_medium t n' m'.zero_le (by simp*)
 
-lemma lift_term2 {l} (t : preterm l) (n n') : (t ↑ n) ↑ n' = t ↑ (n+n') :=
+lemma lift_term2 {l} (t : preterm L l) (n n') : (t ↑ n) ↑ n' = t ↑ (n+n') :=
 lift_term2_medium t n' n.zero_le
 
-lemma lift_term_at2_eq {l} (t : preterm l) (n n' m : ℕ) : 
+lemma lift_term_at2_eq {l} (t : preterm L l) (n n' m : ℕ) : 
   (t ↑' n # m) ↑' n' # (m+n) = t ↑' (n+n') # m :=
 lift_term_at2_medium t n' (m.le_add_right n) (le_refl _)
 
-lemma lift_term_at2_large {l} (t : preterm l) {n} (n') {m m'} (H : m + n ≤ m') : 
+lemma lift_term_at2_large {l} (t : preterm L l) {n} (n') {m m'} (H : m + n ≤ m') : 
   (t ↑' n # m) ↑' n' # m' = (t ↑' n' # (m'-n)) ↑' n # m :=
 have H₁ : n ≤ m', from le_trans (n.le_add_left m) H,
 have H₂ : m ≤ m' - n, from nat.le_sub_right_of_add_le H,
 begin rw fol.lift_term_at2_small t n' n H₂, rw [nat.sub_add_cancel], exact H₁ end
 
-@[simp] lemma lift_term_var0 (n : ℕ) : &0 ↑ n = (&n : term) := 
+@[simp] lemma lift_term_var0 (n : ℕ) : &0 ↑ n = (&n : term L) := 
 by have h : 0 ≤ 0 := le_refl 0; rw [←lift_term_def]; simp [h, -lift_term_def]
 
 /- subst_term t s n substitutes s for (&n) and reduces the level of all variables above n by 1 -/
-def subst_term : ∀ {l}, preterm l → term → ℕ → preterm l
+def subst_term : ∀ {l}, preterm L l → term L → ℕ → preterm L l
 | _ &k          s n := subst_realize var (s ↑ n) n k
 | _ (func f)    s n := func f
 | _ (app t₁ t₂) s n := app (subst_term t₁ s n) (subst_term t₂ s n)
 
 notation t `[`:max s ` // `:95 n `]`:0 := _root_.fol.subst_term t s n
 
-@[simp] lemma subst_term_var_lt (s : term) {k n : ℕ} (H : k < n) : &k[s // n] = &k :=
+@[simp] lemma subst_term_var_lt (s : term L) {k n : ℕ} (H : k < n) : &k[s // n] = &k :=
 by simp only [H, fol.subst_term, fol.subst_realize_lt, eq_self_iff_true]
 
-@[simp] lemma subst_term_var_gt (s : term) {k n : ℕ} (H : n < k) : &k[s // n] = &(k-1) :=
+@[simp] lemma subst_term_var_gt (s : term L) {k n : ℕ} (H : n < k) : &k[s // n] = &(k-1) :=
 by simp only [H, fol.subst_term, fol.subst_realize_gt, eq_self_iff_true]
 
-@[simp] lemma subst_term_var_eq (s : term) (n : ℕ) : &n[s // n] = s ↑' n # 0 :=
+@[simp] lemma subst_term_var_eq (s : term L) (n : ℕ) : &n[s // n] = s ↑' n # 0 :=
 by simp [subst_term]
 
-lemma subst_term_var0 (s : term) : &0[s // 0] = s := by simp
+lemma subst_term_var0 (s : term L) : &0[s // 0] = s := by simp
 
-@[simp] lemma subst_term_func {l} (f : L.functions l) (s : term) (n : ℕ) : 
+@[simp] lemma subst_term_func {l} (f : L.functions l) (s : term L) (n : ℕ) : 
   (func f)[s // n] = func f :=
 by refl
 
-@[simp] lemma subst_term_app {l} (t₁ : preterm (l+1)) (t₂ s : term) (n : ℕ) : 
+@[simp] lemma subst_term_app {l} (t₁ : preterm L (l+1)) (t₂ s : term L) (n : ℕ) : 
   (app t₁ t₂)[s // n] = app (t₁[s // n]) (t₂[s // n]) :=
 by refl
 
-@[simp] lemma subst_term_apps {l} (t : preterm l) (ts : dvector term l) (s : term) (n : ℕ) : 
+@[simp] lemma subst_term_apps {l} (t : preterm L l) (ts : dvector (term L) l) (s : term L) (n : ℕ) : 
   (apps t ts)[s // n] = apps (t[s // n]) (ts.map $ λx, x[s // n]) :=
 begin
   induction ts generalizing t, refl, apply ts_ih (app t ts_x)
@@ -289,7 +289,7 @@ end
 
 /- the following lemmas simplify first lifting and then substituting, depending on the size
   of the substituted variable -/
-lemma lift_at_subst_term_large : ∀{l} (t : preterm l) (s : term) {n₁} (n₂) {m}, m ≤ n₁ →
+lemma lift_at_subst_term_large : ∀{l} (t : preterm L l) (s : term L) {n₁} (n₂) {m}, m ≤ n₁ →
  (t ↑' n₂ # m)[s // n₁+n₂] = (t [s // n₁]) ↑' n₂ # m
 | _ &k          s n₁ n₂ m h :=
   begin
@@ -306,15 +306,15 @@ lemma lift_at_subst_term_large : ∀{l} (t : preterm l) (s : term) {n₁} (n₂)
 | _ (func f)    s n₁ n₂ m h := rfl
 | _ (app t₁ t₂) s n₁ n₂ m h := by simp*
 
-lemma lift_subst_term_large {l} (t : preterm l) (s : term) (n₁ n₂) :
+lemma lift_subst_term_large {l} (t : preterm L l) (s : term L) (n₁ n₂) :
   (t ↑ n₂)[s // n₁+n₂] = (t [s // n₁]) ↑ n₂ :=
 lift_at_subst_term_large t s n₂ n₁.zero_le
 
-lemma lift_subst_term_large' {l} (t : preterm l) (s : term) (n₁ n₂) :
+lemma lift_subst_term_large' {l} (t : preterm L l) (s : term L) (n₁ n₂) :
   (t ↑ n₂)[s // n₂+n₁] = (t [s // n₁]) ↑ n₂ :=
 by rw [add_comm]; apply lift_subst_term_large
 
-lemma lift_at_subst_term_medium : ∀{l} (t : preterm l) (s : term) {n₁ n₂ m}, m ≤ n₂ → 
+lemma lift_at_subst_term_medium : ∀{l} (t : preterm L l) (s : term L) {n₁ n₂ m}, m ≤ n₂ → 
   n₂ ≤ m + n₁ → (t ↑' n₁+1 # m)[s // n₂] = t ↑' n₁ # m
 | _ &k          s n₁ n₂ m h₁ h₂ := 
   begin 
@@ -326,17 +326,17 @@ lemma lift_at_subst_term_medium : ∀{l} (t : preterm l) (s : term) {n₁ n₂ m
 | _ (func f)    s n₁ n₂ m h₁ h₂ := rfl
 | _ (app t₁ t₂) s n₁ n₂ m h₁ h₂ := by simp*
 
-lemma lift_subst_term_medium {l} (t : preterm l) (s : term) (n₁ n₂) :
+lemma lift_subst_term_medium {l} (t : preterm L l) (s : term L) (n₁ n₂) :
   (t ↑ ((n₁ + n₂) + 1))[s // n₁] = t ↑ (n₁ + n₂) :=
 lift_at_subst_term_medium t s n₁.zero_le (by rw [zero_add]; exact n₁.le_add_right n₂)
 
-lemma lift_at_subst_term_eq {l} (t : preterm l) (s : term) (n : ℕ) : (t ↑' 1 # n)[s // n] = t :=
+lemma lift_at_subst_term_eq {l} (t : preterm L l) (s : term L) (n : ℕ) : (t ↑' 1 # n)[s // n] = t :=
 begin rw [lift_at_subst_term_medium t s, lift_term_at_zero]; refl end
 
-@[simp] lemma lift_term1_subst_term {l} (t : preterm l) (s : term) : (t ↑ 1)[s // 0] = t :=
+@[simp] lemma lift_term1_subst_term {l} (t : preterm L l) (s : term L) : (t ↑ 1)[s // 0] = t :=
 lift_at_subst_term_eq t s 0
 
-lemma lift_at_subst_term_small : ∀{l} (t : preterm l) (s : term) (n₁ n₂ m), 
+lemma lift_at_subst_term_small : ∀{l} (t : preterm L l) (s : term L) (n₁ n₂ m), 
  (t ↑' n₁ # (m + n₂ + 1))[s ↑' n₁ # m // n₂] = (t [s // n₂]) ↑' n₁ # (m + n₂)
 | _ &k          s n₁ n₂ m := 
   begin
@@ -361,7 +361,7 @@ lemma lift_at_subst_term_small : ∀{l} (t : preterm l) (s : term) (n₁ n₂ m)
 | _ (func f)    s n₁ n₂ m := rfl
 | _ (app t₁ t₂) s n₁ n₂ m := by simp [*, -add_assoc, -add_comm]
 
-lemma subst_term2 : ∀{l} (t : preterm l) (s₁ s₂ : term) (n₁ n₂),
+lemma subst_term2 : ∀{l} (t : preterm L l) (s₁ s₂ : term L) (n₁ n₂),
   t [s₁ // n₁] [s₂ // n₁ + n₂] = t [s₂ // n₁ + n₂ + 1] [s₁[s₂ // n₂] // n₁]
 | _ &k          s₁ s₂ n₁ n₂ :=
   begin -- can we use subst_realize2 here?
@@ -382,11 +382,11 @@ lemma subst_term2 : ∀{l} (t : preterm l) (s₁ s₂ : term) (n₁ n₂),
 | _ (func f)    s₁ s₂ n₁ n₂ := rfl
 | _ (app t₁ t₂) s₁ s₂ n₁ n₂ := by simp*
 
-lemma subst_term2_0 {l} (t : preterm l) (s₁ s₂ : term) (n) :
+lemma subst_term2_0 {l} (t : preterm L l) (s₁ s₂ : term L) (n) :
   t [s₁ // 0] [s₂ // n] = t [s₂ // n + 1] [s₁[s₂ // n] // 0] :=
 let h := subst_term2 t s₁ s₂ 0 n in by simp only [zero_add] at h; exact h
 
-lemma lift_subst_term_cancel : ∀{l} (t : preterm l) (n : ℕ), (t ↑' 1 # (n+1))[&0 // n] = t
+lemma lift_subst_term_cancel : ∀{l} (t : preterm L l) (n : ℕ), (t ↑' 1 # (n+1))[&0 // n] = t
 | _ &k          n :=
   begin
     apply lt_by_cases n k; intro h, 
@@ -413,50 +413,50 @@ subst_is_lift : (forall N T A n j, N [n ← T]=A↑' 1#j->j<n->exists M,N=M↑' 
   * Similarly, universal quantification is our only quantifier. 
   * We could make `falsum` and `equal` into elements of rel. However, if we do that, then we cannot make the interpretation of them in a model definitionally what we want.
 -/
-parameter (L)
+variable (L)
 inductive preformula : ℕ → Type u
 | falsum {} : preformula 0
-| equal (t₁ t₂ : term) : preformula 0
+| equal (t₁ t₂ : term L) : preformula 0
 | rel {l : ℕ} (R : L.relations l) : preformula l
-| apprel {l : ℕ} (f : preformula (l + 1)) (t : term) : preformula l
+| apprel {l : ℕ} (f : preformula (l + 1)) (t : term L) : preformula l
 | imp (f₁ f₂ : preformula 0) : preformula 0
 | all (f : preformula 0) : preformula 0
 export preformula
-@[reducible] def formula := preformula 0
-parameter {L}
+@[reducible] def formula := preformula L 0
+variable {L}
 
 notation `⊥` := _root_.fol.preformula.falsum -- input: \bot
 infix ` ≃ `:88 := _root_.fol.preformula.equal -- input \~- or \simeq
 infix ` ⟹ `:62 := _root_.fol.preformula.imp -- input \==>
 prefix `∀'`:110 := _root_.fol.preformula.all
-def not (f : formula) : formula := imp f ⊥
+def not (f : formula L) : formula L := imp f ⊥
 prefix `∼`:max := _root_.fol.not -- input \~, the ASCII character ~ has too low precedence
-def and (f₁ f₂ : formula) : formula := ∼(f₁ ⟹ ∼f₂)
+def and (f₁ f₂ : formula L) : formula L := ∼(f₁ ⟹ ∼f₂)
 infixr ` ⊓ ` := _root_.fol.and -- input: \sqcap
-def or (f₁ f₂ : formula) : formula := ∼f₁ ⟹ f₂
+def or (f₁ f₂ : formula L) : formula L := ∼f₁ ⟹ f₂
 infixr ` ⊔ ` := _root_.fol.or -- input: \sqcup
-def biimp (f₁ f₂ : formula) : formula := (f₁ ⟹ f₂) ⊓ (f₂ ⟹ f₁)
+def biimp (f₁ f₂ : formula L) : formula L := (f₁ ⟹ f₂) ⊓ (f₂ ⟹ f₁)
 infix ` ⇔ `:61 := _root_.fol.biimp -- input \<=>
-def ex (f : formula) : formula := ∼ ∀' ∼f
+def ex (f : formula L) : formula L := ∼ ∀' ∼f
 prefix `∃'`:110 := _root_.fol.ex
 
-def apps_rel : ∀{l} (f : preformula l) (ts : dvector term l), formula
+def apps_rel : ∀{l} (f : preformula L l) (ts : dvector (term L) l), formula L
 | 0     f []      := f
 | (n+1) f (t::ts) := apps_rel (apprel f t) ts
 
-@[simp] lemma apps_rel_zero (f : formula) (ts : dvector term 0) : apps_rel f ts = f :=
+@[simp] lemma apps_rel_zero (f : formula L) (ts : dvector (term L) 0) : apps_rel f ts = f :=
 by cases ts; refl
 
-def formula_of_relation {l} (R : L.relations l) : arity term formula l :=
+def formula_of_relation {l} (R : L.relations l) : arity (term L) (formula L) l :=
 arity.of_dvector_map $ apps_rel (rel R)
 
-def formula.rec {C : formula → Sort v}
+def formula.rec {C : formula L → Sort v}
   (hfalsum : C ⊥)
-  (hequal : Π (t₁ t₂ : term), C (t₁ ≃ t₂))
-  (hrel : Π {l} (R : L.relations l) (ts : dvector term l), C (apps_rel (rel R) ts))
-  (himp : Π {{f₁ f₂ : formula}} (ih₁ : C f₁) (ih₂ : C f₂), C (f₁ ⟹ f₂))
-  (hall : Π {{f : formula}} (ih : C f), C (∀' f)) : ∀f, C f :=
-have h : ∀{l} (f : preformula l) (ts : dvector term l), C (apps_rel f ts),
+  (hequal : Π (t₁ t₂ : term L), C (t₁ ≃ t₂))
+  (hrel : Π {l} (R : L.relations l) (ts : dvector (term L) l), C (apps_rel (rel R) ts))
+  (himp : Π {{f₁ f₂ : formula L}} (ih₁ : C f₁) (ih₂ : C f₂), C (f₁ ⟹ f₂))
+  (hall : Π {{f : formula L}} (ih : C f), C (∀' f)) : ∀f, C f :=
+have h : ∀{l} (f : preformula L l) (ts : dvector (term L) l), C (apps_rel f ts),
 begin
   intros, induction f; try {rw ts.zero_eq},
   exact hfalsum, apply hequal, apply hrel, apply f_ih (f_t::ts),
@@ -464,7 +464,7 @@ begin
 end,
 λ f, h f ([])
 
-@[simp] def lift_formula_at : ∀ {l}, preformula l → ℕ → ℕ → preformula l
+@[simp] def lift_formula_at : ∀ {l}, preformula L l → ℕ → ℕ → preformula L l
 | _ falsum       n m := falsum
 | _ (t₁ ≃ t₂)    n m := lift_term_at t₁ n m ≃ lift_term_at t₂ n m
 | _ (rel R)      n m := rel R
@@ -474,14 +474,14 @@ end,
 
 notation f ` ↑' `:90 n ` # `:90 m:90 := _root_.fol.lift_formula_at f n m -- input ↑' with \upa
 
-@[reducible] def lift_formula {l} (f : preformula l) (n : ℕ) : preformula l := f ↑' n # 0
+@[reducible] def lift_formula {l} (f : preformula L l) (n : ℕ) : preformula L l := f ↑' n # 0
 infix ` ↑ `:100 := _root_.fol.lift_formula -- input ↑' with \upa
-@[reducible, simp] def lift_formula1 {l} (f : preformula l) : preformula l := f ↑ 1
+@[reducible, simp] def lift_formula1 {l} (f : preformula L l) : preformula L l := f ↑ 1
 
-@[simp] lemma lift_formula_def {l} (f : preformula l) (n : ℕ) : f ↑' n # 0 = f ↑ n := by refl
-@[simp] lemma lift_formula1_not (n : ℕ) (f : formula) : ∼f ↑ n  = ∼(f ↑ n) := by refl
+@[simp] lemma lift_formula_def {l} (f : preformula L l) (n : ℕ) : f ↑' n # 0 = f ↑ n := by refl
+@[simp] lemma lift_formula1_not (n : ℕ) (f : formula L) : ∼f ↑ n  = ∼(f ↑ n) := by refl
 
-lemma lift_formula_at_inj {l} {f f' : preformula l} {n m : ℕ} (H : f ↑' n # m = f' ↑' n # m) : 
+lemma lift_formula_at_inj {l} {f f' : preformula L l} {n m : ℕ} (H : f ↑' n # m = f' ↑' n # m) : 
   f = f' :=
 begin
   induction f generalizing m; cases f'; injection H,
@@ -491,7 +491,7 @@ begin
   { simp only [f_ih h_1, eq_self_iff_true] }
 end
 
-@[simp] lemma lift_formula_at_zero : ∀ {l} (f : preformula l) (m : ℕ), f ↑' 0 # m = f
+@[simp] lemma lift_formula_at_zero : ∀ {l} (f : preformula L l) (m : ℕ), f ↑' 0 # m = f
 | _ falsum       m := by refl
 | _ (t₁ ≃ t₂)    m := by simp
 | _ (rel R)      m := by refl
@@ -500,7 +500,7 @@ end
 | _ (∀' f)       m := by simp; apply lift_formula_at_zero
 
 /- the following lemmas simplify iterated lifts, depending on the size of m' -/
-lemma lift_formula_at2_small : ∀ {l} (f : preformula l) (n n') {m m'}, m' ≤ m → 
+lemma lift_formula_at2_small : ∀ {l} (f : preformula L l) (n n') {m m'}, m' ≤ m → 
   (f ↑' n # m) ↑' n' # m' = (f ↑' n' # m') ↑' n # (m + n')
 | _ falsum       n n' m m' H := by refl
 | _ (t₁ ≃ t₂)    n n' m m' H := by simp [lift_term_at2_small, H]
@@ -511,7 +511,7 @@ lemma lift_formula_at2_small : ∀ {l} (f : preformula l) (n n') {m m'}, m' ≤ 
 | _ (∀' f)       n n' m m' H :=
   by simp [lift_term_at2_small, H, lift_formula_at2_small f n n' (add_le_add_right H 1)]
 
-lemma lift_formula_at2_medium : ∀ {l} (f : preformula l) (n n') {m m'}, m ≤ m' → m' ≤ m+n → 
+lemma lift_formula_at2_medium : ∀ {l} (f : preformula L l) (n n') {m m'}, m ≤ m' → m' ≤ m+n → 
   (f ↑' n # m) ↑' n' # m' = f ↑' (n+n') # m
 | _ falsum       n n' m m' H₁ H₂ := by refl
 | _ (t₁ ≃ t₂)    n n' m m' H₁ H₂ := by simp [*, lift_term_at2_medium]
@@ -521,17 +521,17 @@ lemma lift_formula_at2_medium : ∀ {l} (f : preformula l) (n n') {m m'}, m ≤ 
 | _ (∀' f)       n n' m m' H₁ H₂ :=
   have m' + 1 ≤ (m + 1) + n, from le_trans (add_le_add_right H₂ 1) (by simp), by simp*
 
-lemma lift_formula_at2_eq {l} (f : preformula l) (n n' m : ℕ) : 
+lemma lift_formula_at2_eq {l} (f : preformula L l) (n n' m : ℕ) : 
   (f ↑' n # m) ↑' n' # (m+n) = f ↑' (n+n') # m :=
 lift_formula_at2_medium f n n' (m.le_add_right n) (le_refl _)
 
-lemma lift_formula_at2_large {l} (f : preformula l) (n n') {m m'} (H : m + n ≤ m') : 
+lemma lift_formula_at2_large {l} (f : preformula L l) (n n') {m m'} (H : m + n ≤ m') : 
   (f ↑' n # m) ↑' n' # m' = (f ↑' n' # (m'-n)) ↑' n # m :=
 have H₁ : n ≤ m', from le_trans (n.le_add_left m) H,
 have H₂ : m ≤ m' - n, from nat.le_sub_right_of_add_le H,
 begin rw lift_formula_at2_small f n' n H₂, rw [nat.sub_add_cancel], exact H₁ end
 
-@[simp] def subst_formula : ∀ {l}, preformula l → term → ℕ → preformula l
+@[simp] def subst_formula : ∀ {l}, preformula L l → term L → ℕ → preformula L l
 | _ falsum       s n := falsum
 | _ (t₁ ≃ t₂)    s n := subst_term t₁ s n ≃ subst_term t₂ s n
 | _ (rel R)      s n := rel R
@@ -541,21 +541,21 @@ begin rw lift_formula_at2_small f n' n H₂, rw [nat.sub_add_cancel], exact H₁
 
 notation f `[`:95 s ` // `:95 n `]`:0 := _root_.fol.subst_formula f s n
 
-lemma subst_formula_equal (t₁ t₂ s : term) (n : ℕ) :
+lemma subst_formula_equal (t₁ t₂ s : term L) (n : ℕ) :
   (t₁ ≃ t₂)[s // n] = t₁[s // n] ≃ (t₂[s // n]) :=
 by refl
 
-@[simp] lemma subst_formula_biimp (f₁ f₂ : formula) (s : term) (n : ℕ) :
+@[simp] lemma subst_formula_biimp (f₁ f₂ : formula L) (s : term L) (n : ℕ) :
   (f₁ ⇔ f₂)[s // n] = f₁[s // n] ⇔ (f₂[s // n]) :=
 by refl
 
-@[simp] lemma subst_formula_apps_rel {l} (f : preformula l) (ts : dvector term l) (s : term) 
+@[simp] lemma subst_formula_apps_rel {l} (f : preformula L l) (ts : dvector (term L) l) (s : term L) 
   (n : ℕ): (apps_rel f ts)[s // n] = apps_rel (f[s // n]) (ts.map $ λx, x[s // n]) :=
 begin
   induction ts generalizing f, refl, apply ts_ih (apprel f ts_x)
 end
 
-lemma lift_at_subst_formula_large : ∀{l} (f : preformula l) (s : term) {n₁} (n₂) {m}, m ≤ n₁ →
+lemma lift_at_subst_formula_large : ∀{l} (f : preformula L l) (s : term L) {n₁} (n₂) {m}, m ≤ n₁ →
   (f ↑' n₂ # m)[s // n₁+n₂] = (f [s // n₁]) ↑' n₂ # m
 | _ falsum       s n₁ n₂ m h := by refl
 | _ (t₁ ≃ t₂)    s n₁ n₂ m h := by simp [*, lift_at_subst_term_large]
@@ -565,15 +565,15 @@ lemma lift_at_subst_formula_large : ∀{l} (f : preformula l) (s : term) {n₁} 
 | _ (∀' f)       s n₁ n₂ m h := 
   by have := lift_at_subst_formula_large f s n₂ (add_le_add_right h 1); simp at this; simp*
 
-lemma lift_subst_formula_large {l} (f : preformula l) (s : term) {n₁ n₂} :
+lemma lift_subst_formula_large {l} (f : preformula L l) (s : term L) {n₁ n₂} :
   (f ↑ n₂)[s // n₁+n₂] = (f [s // n₁]) ↑ n₂ :=
 lift_at_subst_formula_large f s n₂ n₁.zero_le
 
-lemma lift_subst_formula_large' {l} (f : preformula l) (s : term) {n₁ n₂} :
+lemma lift_subst_formula_large' {l} (f : preformula L l) (s : term L) {n₁ n₂} :
   (f ↑ n₂)[s // n₂+n₁] = (f [s // n₁]) ↑ n₂ :=
 by rw [add_comm]; apply lift_subst_formula_large
 
-lemma lift_at_subst_formula_medium : ∀{l} (f : preformula l) (s : term) {n₁ n₂ m}, m ≤ n₂ → 
+lemma lift_at_subst_formula_medium : ∀{l} (f : preformula L l) (s : term L) {n₁ n₂ m}, m ≤ n₂ → 
   n₂ ≤ m + n₁ → (f ↑' n₁+1 # m)[s // n₂] = f ↑' n₁ # m
 | _ falsum       s n₁ n₂ m h₁ h₂ := by refl
 | _ (t₁ ≃ t₂)    s n₁ n₂ m h₁ h₂ := by simp [*, lift_at_subst_term_medium]
@@ -587,18 +587,18 @@ lemma lift_at_subst_formula_medium : ∀{l} (f : preformula l) (s : term) {n₁ 
     simp only [fol.subst_formula, fol.lift_formula_at] at this, simp*
   end
 
-lemma lift_subst_formula_medium {l} (f : preformula l) (s : term) (n₁ n₂) :
+lemma lift_subst_formula_medium {l} (f : preformula L l) (s : term L) (n₁ n₂) :
   (f ↑ ((n₁ + n₂) + 1))[s // n₁] = f ↑ (n₁ + n₂) :=
 lift_at_subst_formula_medium f s n₁.zero_le (by rw [zero_add]; exact n₁.le_add_right n₂)
 
-lemma lift_at_subst_formula_eq {l} (f : preformula l) (s : term) (n : ℕ) : 
+lemma lift_at_subst_formula_eq {l} (f : preformula L l) (s : term L) (n : ℕ) : 
   (f ↑' 1 # n)[s // n] = f :=
 begin rw [lift_at_subst_formula_medium f s, lift_formula_at_zero]; refl end
 
-@[simp] lemma lift_formula1_subst {l} (f : preformula l) (s : term) : (f ↑ 1)[s // 0] = f :=
+@[simp] lemma lift_formula1_subst {l} (f : preformula L l) (s : term L) : (f ↑ 1)[s // 0] = f :=
 lift_at_subst_formula_eq f s 0
 
-lemma lift_at_subst_formula_small : ∀{l} (f : preformula l) (s : term) (n₁ n₂ m), 
+lemma lift_at_subst_formula_small : ∀{l} (f : preformula L l) (s : term L) (n₁ n₂ m), 
  (f ↑' n₁ # (m + n₂ + 1))[s ↑' n₁ # m // n₂] = (f [s // n₂]) ↑' n₁ # (m + n₂)
 | _ falsum       s n₁ n₂ m := by refl
 | _ (t₁ ≃ t₂)    s n₁ n₂ m := 
@@ -611,11 +611,11 @@ lemma lift_at_subst_formula_small : ∀{l} (f : preformula l) (s : term) (n₁ n
 | _ (∀' f)       s n₁ n₂ m := 
     by have := lift_at_subst_formula_small f s n₁ (n₂+1) m; dsimp; simp at this ⊢; exact this
 
-lemma lift_at_subst_formula_small0 {l} (f : preformula l) (s : term) (n₁ m) :
+lemma lift_at_subst_formula_small0 {l} (f : preformula L l) (s : term L) (n₁ m) :
  (f ↑' n₁ # (m + 1))[s ↑' n₁ # m // 0] = (f [s // 0]) ↑' n₁ # m :=
 lift_at_subst_formula_small f s n₁ 0 m
 
-lemma subst_formula2 : ∀{l} (f : preformula l) (s₁ s₂ : term) (n₁ n₂),
+lemma subst_formula2 : ∀{l} (f : preformula L l) (s₁ s₂ : term L) (n₁ n₂),
   f [s₁ // n₁] [s₂ // n₁ + n₂] = f [s₂ // n₁ + n₂ + 1] [s₁[s₂ // n₂] // n₁]
 | _ falsum       s₁ s₂ n₁ n₂ := by refl
 | _ (t₁ ≃ t₂)    s₁ s₂ n₁ n₂ := by simp [*, subst_term2]
@@ -625,11 +625,11 @@ lemma subst_formula2 : ∀{l} (f : preformula l) (s₁ s₂ : term) (n₁ n₂),
 | _ (∀' f)       s₁ s₂ n₁ n₂ := 
   by simp*; rw [add_comm n₂ 1, ←add_assoc, subst_formula2 f s₁ s₂ (n₁ + 1) n₂]; simp
 
-lemma subst_formula2_zero {l} (f : preformula l) (s₁ s₂ : term) (n) :
+lemma subst_formula2_zero {l} (f : preformula L l) (s₁ s₂ : term L) (n) :
   f [s₁ // 0] [s₂ // n] = f [s₂ // n + 1] [s₁[s₂ // n] // 0] :=
 let h := subst_formula2 f s₁ s₂ 0 n in by simp only [fol.subst_formula, zero_add] at h; exact h
 
-lemma lift_subst_formula_cancel : ∀{l} (f : preformula l) (n : ℕ), (f ↑' 1 # (n+1))[&0 // n] = f
+lemma lift_subst_formula_cancel : ∀{l} (f : preformula L l) (n : ℕ), (f ↑' 1 # (n+1))[&0 // n] = f
 | _ falsum       n := by refl
 | _ (t₁ ≃ t₂)    n := by simp [*, lift_subst_term_cancel]
 | _ (rel R)      n := by refl
@@ -637,7 +637,7 @@ lemma lift_subst_formula_cancel : ∀{l} (f : preformula l) (n : ℕ), (f ↑' 1
 | _ (f₁ ⟹ f₂)   n := by simp*
 | _ (∀' f)       n := by simp*
 
-@[simp] def count_quantifiers : ∀ {l}, preformula l → ℕ
+@[simp] def count_quantifiers : ∀ {l}, preformula L l → ℕ
 | _ falsum       := 0
 | _ (t₁ ≃ t₂)    := 0
 | _ (rel R)      := 0
@@ -645,10 +645,10 @@ lemma lift_subst_formula_cancel : ∀{l} (f : preformula l) (n : ℕ), (f ↑' 1
 | _ (f₁ ⟹ f₂)   := count_quantifiers f₁ + count_quantifiers f₂
 | _ (∀' f)       := count_quantifiers f + 1
 
-@[simp] def count_quantifiers_succ {l} (f : preformula (l+1)) : count_quantifiers f = 0 :=
+@[simp] def count_quantifiers_succ {l} (f : preformula L (l+1)) : count_quantifiers f = 0 :=
 by cases f; refl
 
-@[simp] lemma count_quantifiers_subst : ∀ {l} (f : preformula l) (s : term) (n : ℕ),
+@[simp] lemma count_quantifiers_subst : ∀ {l} (f : preformula L l) (s : term L) (n : ℕ),
   count_quantifiers (f[s // n]) = count_quantifiers f
 | _ falsum       s n := by refl
 | _ (t₁ ≃ t₂)    s n := by refl
@@ -662,34 +662,34 @@ by cases f; refl
 * We use natural deduction as our deduction system, since that is most convenient to work with.
 * All rules are motivated to work well with backwards reasoning.
 -/
-inductive prf : set formula → formula → Type u
+inductive prf : set (formula L) → formula L → Type u
 | axm     {Γ A} (h : A ∈ Γ) : prf Γ A
-| impI    {Γ : set formula} {A B} (h : prf (insert A Γ) B) : prf Γ (A ⟹ B)
+| impI    {Γ : set $ formula L} {A B} (h : prf (insert A Γ) B) : prf Γ (A ⟹ B)
 | impE    {Γ} (A) {B} (h₁ : prf Γ (A ⟹ B)) (h₂ : prf Γ A) : prf Γ B
-| falsumE {Γ : set formula} {A} (h : prf (insert ∼A Γ) falsum) : prf Γ A
+| falsumE {Γ : set $ formula L} {A} (h : prf (insert ∼A Γ) falsum) : prf Γ A
 | allI    {Γ A} (h : prf (lift_formula1 '' Γ) A) : prf Γ (∀' A)
 | allE'   {Γ} A t (h : prf Γ (∀' A)) : prf Γ (A[t // 0])
-| refl    (Γ t) : prf Γ (t ≃ t)
+| ref     (Γ t) : prf Γ (t ≃ t)
 | subst'  {Γ} (s t f) (h₁ : prf Γ (s ≃ t)) (h₂ : prf Γ (f[s // 0])) : prf Γ (f[t // 0])
 
 export prf
 infix ` ⊢ `:51 := _root_.fol.prf -- input: \|- or \vdash
 
-def provable (T : set formula) (f : formula) := nonempty (prf T f)
+def provable (T : set $ formula L) (f : formula L) := nonempty (prf T f)
 infix ` ⊢' `:51 := _root_.fol.provable -- input: \|- or \vdash
 
-def allE {Γ} (A : formula) (t) {B} (H₁ : prf Γ (∀' A)) (H₂ : A[t // 0] = B) : prf Γ B :=
+def allE {Γ} (A : formula L) (t) {B} (H₁ : prf Γ (∀' A)) (H₂ : A[t // 0] = B) : prf Γ B :=
 by induction H₂; exact allE' A t H₁
 
-def subst {Γ} {s t} (f₁ : formula) {f₂} (H₁ : prf Γ (s ≃ t)) (H₂ : prf Γ (f₁[s // 0])) 
+def subst {Γ} {s t} (f₁ : formula L) {f₂} (H₁ : prf Γ (s ≃ t)) (H₂ : prf Γ (f₁[s // 0])) 
   (H₃ : f₁[t // 0] = f₂) : prf Γ f₂ :=
 by induction H₃; exact subst' s t f₁ H₁ H₂
 
-def axm1 {Γ : set formula} {A : formula} : insert A Γ ⊢ A := by apply axm; left; refl
-def axm2 {Γ : set formula} {A B : formula} : insert A (insert B Γ) ⊢ B := 
+def axm1 {Γ : set (formula L)} {A : formula L} : insert A Γ ⊢ A := by apply axm; left; refl
+def axm2 {Γ : set (formula L)} {A B : formula L} : insert A (insert B Γ) ⊢ B := 
 by apply axm; right; left; refl
 
-def weakening {Γ Δ} {f : formula} (H₁ : Γ ⊆ Δ) (H₂ : Γ ⊢ f) : Δ ⊢ f :=
+def weakening {Γ Δ} {f : formula L} (H₁ : Γ ⊆ Δ) (H₂ : Γ ⊢ f) : Δ ⊢ f :=
 begin
   induction H₂ generalizing Δ,
   { apply axm, exact H₁ H₂_h, },
@@ -698,11 +698,11 @@ begin
   { apply falsumE, apply H₂_ih, apply insert_subset_insert, apply H₁ },
   { apply allI, apply H₂_ih, apply image_subset _ H₁ },
   { apply allE', apply H₂_ih, assumption },
-  { apply refl },
+  { apply ref },
   { apply subst', apply H₂_ih_h₁, assumption, apply H₂_ih_h₂, assumption },
 end
 
-def prf_lift {Γ} {f : formula} (n m : ℕ) (H : Γ ⊢ f) : (λf', f' ↑' n # m) '' Γ ⊢ f ↑' n # m :=
+def prf_lift {Γ} {f : formula L} (n m : ℕ) (H : Γ ⊢ f) : (λf', f' ↑' n # m) '' Γ ⊢ f ↑' n # m :=
 begin
   induction H generalizing m,
   { apply axm, apply mem_image_of_mem _ H_h },
@@ -713,13 +713,13 @@ begin
     apply cast _ h, congr1, apply image_congr', intro f', symmetry,
     exact lift_formula_at2_small f' _ _ m.zero_le },
   { apply allE _ _ (H_ih m), apply lift_at_subst_formula_small0 },
-  { apply refl },
+  { apply ref },
   { apply subst _ (H_ih_h₁ m), 
     { have h := @H_ih_h₂ m, rw [←lift_at_subst_formula_small0] at h, exact h},
     rw [lift_at_subst_formula_small0] },
 end
 
-def substitution {Γ} {f : formula} {t n} (H : Γ ⊢ f) : (λx, x[t // n]) '' Γ ⊢ f[t // n] :=
+def substitution {Γ} {f : formula L} {t n} (H : Γ ⊢ f) : (λx, x[t // n]) '' Γ ⊢ f[t // n] :=
 begin
   induction H generalizing n,
   { apply axm, apply mem_image_of_mem _ H_h },
@@ -730,49 +730,49 @@ begin
     apply cast _ h, congr1, apply image_congr', intro,
     apply lift_subst_formula_large },
   { apply allE _ _ H_ih, symmetry, apply subst_formula2_zero },
-  { apply refl },
+  { apply ref },
   { apply subst _ H_ih_h₁, { have h := @H_ih_h₂ n, rw [subst_formula2_zero] at h, exact h}, 
     rw [subst_formula2_zero] },
 end
 
-def weakening1 {Γ} {f₁ f₂ : formula} (H : Γ ⊢ f₂) : insert f₁ Γ ⊢ f₂ :=
+def weakening1 {Γ} {f₁ f₂ : formula L} (H : Γ ⊢ f₂) : insert f₁ Γ ⊢ f₂ :=
 weakening (subset_insert f₁ Γ) H
 
-def weakening2 {Γ} {f₁ f₂ f₃ : formula} (H : insert f₁ Γ ⊢ f₂) : insert f₁ (insert f₃ Γ) ⊢ f₂ :=
+def weakening2 {Γ} {f₁ f₂ f₃ : formula L} (H : insert f₁ Γ ⊢ f₂) : insert f₁ (insert f₃ Γ) ⊢ f₂ :=
 weakening (insert_subset_insert (subset_insert _ Γ)) H
 
-def deduction {Γ} {A B : formula} (H : Γ ⊢ A ⟹ B) : insert A Γ ⊢ B :=
+def deduction {Γ} {A B : formula L} (H : Γ ⊢ A ⟹ B) : insert A Γ ⊢ B :=
 impE A (weakening1 H) axm1
 
-def exfalso {Γ} {A : formula} (H : Γ ⊢ falsum) : prf Γ A :=
+def exfalso {Γ} {A : formula L} (H : Γ ⊢ falsum) : prf Γ A :=
 falsumE (weakening1 H)
 
-def notI {Γ} {A : formula} (H : Γ ⊢ A ⟹ falsum) : prf Γ (not A) :=
+def notI {Γ} {A : formula L} (H : Γ ⊢ A ⟹ falsum) : prf Γ (not A) :=
   by {rw[not], assumption}
 
-def andI {Γ} {f₁ f₂ : formula} (H₁ : Γ ⊢ f₁) (H₂ : Γ ⊢ f₂) : Γ ⊢ f₁ ⊓ f₂ :=
+def andI {Γ} {f₁ f₂ : formula L} (H₁ : Γ ⊢ f₁) (H₂ : Γ ⊢ f₂) : Γ ⊢ f₁ ⊓ f₂ :=
 begin 
   apply impI, apply impE f₂,
   { apply impE f₁, apply axm1, exact weakening1 H₁ },
   { exact weakening1 H₂ }
 end
 
-def andE1 {Γ f₁} (f₂ : formula) (H : Γ ⊢ f₁ ⊓ f₂) : Γ ⊢ f₁ :=
+def andE1 {Γ f₁} (f₂ : formula L) (H : Γ ⊢ f₁ ⊓ f₂) : Γ ⊢ f₁ :=
 begin 
   apply falsumE, apply impE _ (weakening1 H), apply impI, apply exfalso,
   apply impE f₁; [apply axm2, apply axm1]
 end
 
-def andE2 {Γ} (f₁ : formula) {f₂} (H : Γ ⊢ f₁ ⊓ f₂) : Γ ⊢ f₂ :=
+def andE2 {Γ} (f₁ : formula L) {f₂} (H : Γ ⊢ f₁ ⊓ f₂) : Γ ⊢ f₂ :=
 begin apply falsumE, apply impE _ (weakening1 H), apply impI, apply axm2 end
 
-def orI1 {Γ} {A B : formula} (H : Γ ⊢ A) : Γ ⊢ A ⊔ B :=
+def orI1 {Γ} {A B : formula L} (H : Γ ⊢ A) : Γ ⊢ A ⊔ B :=
 begin apply impI, apply exfalso, refine impE _ _ (weakening1 H), apply axm1 end
 
-def orI2 {Γ} {A B : formula} (H : Γ ⊢ B) : Γ ⊢ A ⊔ B :=
+def orI2 {Γ} {A B : formula L} (H : Γ ⊢ B) : Γ ⊢ A ⊔ B :=
 impI $ weakening1 H
 
-def orE {Γ} {A B C : formula} (H₁ : Γ ⊢ A ⊔ B) (H₂ : insert A Γ ⊢ C) (H₃ : insert B Γ ⊢ C) : 
+def orE {Γ} {A B C : formula L} (H₁ : Γ ⊢ A ⊔ B) (H₂ : insert A Γ ⊢ C) (H₃ : insert B Γ ⊢ C) : 
   Γ ⊢ C :=
 begin
   apply falsumE, apply impE C, { apply axm1 },
@@ -781,40 +781,40 @@ begin
   apply impI (impE _ axm2 (weakening2 H₂))
 end
 
-def biimpI {Γ} {f₁ f₂ : formula} (H₁ : insert f₁ Γ ⊢ f₂) (H₂ : insert f₂ Γ ⊢ f₁) : Γ ⊢ f₁ ⇔ f₂ :=
+def biimpI {Γ} {f₁ f₂ : formula L} (H₁ : insert f₁ Γ ⊢ f₂) (H₂ : insert f₂ Γ ⊢ f₁) : Γ ⊢ f₁ ⇔ f₂ :=
 by apply andI; apply impI; assumption
 
-def biimpE1 {Γ} {f₁ f₂ : formula} (H : Γ ⊢ f₁ ⇔ f₂) : insert f₁ Γ ⊢ f₂ := deduction (andE1 _ H)
-def biimpE2 {Γ} {f₁ f₂ : formula} (H : Γ ⊢ f₁ ⇔ f₂) : insert f₂ Γ ⊢ f₁ := deduction (andE2 _ H)
+def biimpE1 {Γ} {f₁ f₂ : formula L} (H : Γ ⊢ f₁ ⇔ f₂) : insert f₁ Γ ⊢ f₂ := deduction (andE1 _ H)
+def biimpE2 {Γ} {f₁ f₂ : formula L} (H : Γ ⊢ f₁ ⇔ f₂) : insert f₂ Γ ⊢ f₁ := deduction (andE2 _ H)
 
-lemma iff_of_biimp {Γ} {f₁ f₂ : formula} (H : Γ ⊢' f₁ ⇔ f₂) : Γ ⊢' f₁ ↔ Γ ⊢' f₂ :=
+lemma iff_of_biimp {Γ} {f₁ f₂ : formula L} (H : Γ ⊢' f₁ ⇔ f₂) : Γ ⊢' f₁ ↔ Γ ⊢' f₂ :=
 ⟨(H.map (andE1 _)).map2 (impE _), (H.map (andE2 _)).map2 (impE _)⟩ 
 
-def exI {Γ f} (t : term) (H : Γ ⊢ f [t // 0]) : Γ ⊢ ∃' f :=
+def exI {Γ f} (t : term L) (H : Γ ⊢ f [t // 0]) : Γ ⊢ ∃' f :=
 begin
   apply impI, 
   apply impE (f[t // 0]) _ (weakening1 H),
   apply allE' ∼f t axm1,
 end
 
-def exE {Γ f₁ f₂} (t : term) (H₁ : Γ ⊢ ∃' f₁) 
+def exE {Γ} {f₁ f₂ : formula L} (t : term L) (H₁ : Γ ⊢ ∃' f₁) 
   (H₂ : insert f₁ (lift_formula1 '' Γ) ⊢ lift_formula1 f₂) : Γ ⊢ f₂ :=
 begin
   apply falsumE, apply impE _ (weakening1 H₁), apply allI, apply impI, 
   rw [image_insert_eq], apply impE _ axm2, apply weakening2 H₂
 end
 
-def ex_not_of_not_all {Γ} {f : formula} (H : Γ ⊢ ∼ ∀' f) : Γ ⊢ ∃' ∼ f :=
+def ex_not_of_not_all {Γ} {f : formula L} (H : Γ ⊢ ∼ ∀' f) : Γ ⊢ ∃' ∼ f :=
 begin
   apply falsumE, apply impE _ (weakening1 H), apply allI, apply falsumE,
   rw [image_insert_eq], apply impE _ axm2, apply exI &0,
   rw [lift_subst_formula_cancel], exact axm1
 end
 
-def not_and_self {Γ : set formula} {f : formula} (H : Γ ⊢ f ⊓ ∼f) : Γ ⊢ ⊥ :=
+def not_and_self {Γ : set (formula L)} {f : formula L} (H : Γ ⊢ f ⊓ ∼f) : Γ ⊢ ⊥ :=
 impE f (andE2 f H) (andE1 ∼f H)
 
-lemma prf_all_iff {Γ : set formula} {f} : Γ ⊢' ∀' f ↔ lift_formula1 '' Γ ⊢' f :=
+lemma prf_all_iff {Γ : set (formula L)} {f} : Γ ⊢' ∀' f ↔ lift_formula1 '' Γ ⊢' f :=
 begin
   split,
   { intro H, rw [←lift_subst_formula_cancel f 0], 
@@ -822,59 +822,59 @@ begin
   { exact nonempty.map allI }
 end
 
--- def andE1 {Γ f₁} (f₂ : formula) (H : Γ ⊢ f₁ ⊓ f₂) : Γ ⊢ f₁ :=
-def symm {Γ} {s t : term} (H : Γ ⊢ s ≃ t) : Γ ⊢ t ≃ s :=
+-- def andE1 {Γ f₁} (f₂ : formula L) (H : Γ ⊢ f₁ ⊓ f₂) : Γ ⊢ f₁ :=
+def symm {Γ} {s t : term L} (H : Γ ⊢ s ≃ t) : Γ ⊢ t ≃ s :=
 begin 
   apply subst (&0 ≃ s ↑ 1) H; rw [subst_formula_equal, lift_term1_subst_term, subst_term_var0],
-  apply refl
+  apply ref
 end
 
-def trans {Γ} {t₁ t₂ t₃ : term} (H : Γ ⊢ t₁ ≃ t₂) (H' : Γ ⊢ t₂ ≃ t₃) : Γ ⊢ t₁ ≃ t₃ :=
+def trans {Γ} {t₁ t₂ t₃ : term L} (H : Γ ⊢ t₁ ≃ t₂) (H' : Γ ⊢ t₂ ≃ t₃) : Γ ⊢ t₁ ≃ t₃ :=
 begin 
   apply subst (t₁ ↑ 1 ≃ &0) H'; rw [subst_formula_equal, lift_term1_subst_term, subst_term_var0],
   exact H
 end
 
-def congr {Γ} {t₁ t₂ : term} (s : term) (H : Γ ⊢ t₁ ≃ t₂) : Γ ⊢ s[t₁ // 0] ≃ s[t₂ // 0] :=
+def congr {Γ} {t₁ t₂ : term L} (s : term L) (H : Γ ⊢ t₁ ≃ t₂) : Γ ⊢ s[t₁ // 0] ≃ s[t₂ // 0] :=
 begin 
   apply subst (s[t₁ // 0] ↑ 1 ≃ s) H, 
-  { rw [subst_formula_equal, lift_term1_subst_term], apply refl },
+  { rw [subst_formula_equal, lift_term1_subst_term], apply ref },
   { rw [subst_formula_equal, lift_term1_subst_term] }
 end
 
-def app_congr {Γ} {t₁ t₂ : term} (s : preterm 1) (H : Γ ⊢ t₁ ≃ t₂) : Γ ⊢ app s t₁ ≃ app s t₂ :=
+def app_congr {Γ} {t₁ t₂ : term L} (s : preterm L 1) (H : Γ ⊢ t₁ ≃ t₂) : Γ ⊢ app s t₁ ≃ app s t₂ :=
 begin 
   have h := congr (app (s ↑ 1) &0) H, simp at h, exact h
 end
 
-def apprel_congr {Γ} {t₁ t₂ : term} (f : preformula 1) (H : Γ ⊢ t₁ ≃ t₂)
+def apprel_congr {Γ} {t₁ t₂ : term L} (f : preformula L 1) (H : Γ ⊢ t₁ ≃ t₂)
   (H₂ : Γ ⊢ apprel f t₁) : Γ ⊢ apprel f t₂ :=
 begin 
   apply subst (apprel (f ↑ 1) &0) H; simp, exact H₂
 end
 
-lemma apprel_congr' {Γ} {t₁ t₂ : term} (f : preformula 1) (H : Γ ⊢ t₁ ≃ t₂) :
+lemma apprel_congr' {Γ} {t₁ t₂ : term L} (f : preformula L 1) (H : Γ ⊢ t₁ ≃ t₂) :
   Γ ⊢' apprel f t₁ ↔ Γ ⊢' apprel f t₂ :=
 ⟨nonempty.map $ apprel_congr f H, nonempty.map $ apprel_congr f $ symm H⟩
 
-def imp_trans {Γ} {f₁ f₂ f₃ : formula} (H₁ : Γ ⊢ f₁ ⟹ f₂) (H₂ : Γ ⊢ f₂ ⟹ f₃) : Γ ⊢ f₁ ⟹ f₃ :=
+def imp_trans {Γ} {f₁ f₂ f₃ : formula L} (H₁ : Γ ⊢ f₁ ⟹ f₂) (H₂ : Γ ⊢ f₂ ⟹ f₃) : Γ ⊢ f₁ ⟹ f₃ :=
 begin
   apply impI, apply impE _ (weakening1 H₂), apply impE _ (weakening1 H₁) axm1
 end
 
-def biimp_refl (Γ : set formula) (f : formula) : Γ ⊢ f ⇔ f :=
+def biimp_refl (Γ : set (formula L)) (f : formula L) : Γ ⊢ f ⇔ f :=
 by apply biimpI; apply axm1
 
-def biimp_trans {Γ} {f₁ f₂ f₃ : formula} (H₁ : Γ ⊢ f₁ ⇔ f₂) (H₂ : Γ ⊢ f₂ ⇔ f₃) : Γ ⊢ f₁ ⇔ f₃ :=
+def biimp_trans {Γ} {f₁ f₂ f₃ : formula L} (H₁ : Γ ⊢ f₁ ⇔ f₂) (H₂ : Γ ⊢ f₂ ⇔ f₃) : Γ ⊢ f₁ ⇔ f₃ :=
 begin
   apply andI; apply imp_trans, 
   apply andE1 _ H₁, apply andE1 _ H₂, apply andE2 _ H₂, apply andE2 _ H₁
 end
 
-def equal_preterms (T : set formula) {l} (t₁ t₂ : preterm l) : Type u :=
-∀(ts : dvector term l), T ⊢ apps t₁ ts ≃ apps t₂ ts
+def equal_preterms (T : set (formula L)) {l} (t₁ t₂ : preterm L l) : Type u :=
+∀(ts : dvector (term L) l), T ⊢ apps t₁ ts ≃ apps t₂ ts
 
-def equal_preterms_app {T : set formula} {l} {t t' : preterm (l+1)} {s s' : term} 
+def equal_preterms_app {T : set (formula L)} {l} {t t' : preterm L (l+1)} {s s' : term L} 
   (Ht : equal_preterms T t t') (Hs : T ⊢ s ≃ s') : equal_preterms T (app t s) (app t' s') :=
 begin
   intro xs,
@@ -884,13 +884,13 @@ begin
   exact h
 end
 
-@[refl] def equal_preterms_refl (T : set formula) {l} (t : preterm l) : equal_preterms T t t :=
-λxs, refl T (apps t xs)
+@[refl] def equal_preterms_refl (T : set (formula L)) {l} (t : preterm L l) : equal_preterms T t t :=
+λxs, ref T (apps t xs)
 
-def equiv_preformulae (T : set formula) {l} (f₁ f₂ : preformula l) : Type u :=
-∀(ts : dvector term l), T ⊢ apps_rel f₁ ts ⇔ apps_rel f₂ ts
+def equiv_preformulae (T : set (formula L)) {l} (f₁ f₂ : preformula L l) : Type u :=
+∀(ts : dvector (term L) l), T ⊢ apps_rel f₁ ts ⇔ apps_rel f₂ ts
 
-def equiv_preformulae_apprel {T : set formula} {l} {f f' : preformula (l+1)} {s s' : term} 
+def equiv_preformulae_apprel {T : set (formula L)} {l} {f f' : preformula L (l+1)} {s s' : term L} 
   (Ht : equiv_preformulae T f f') (Hs : T ⊢ s ≃ s') : 
     equiv_preformulae T (apprel f s) (apprel f' s') :=
 begin
@@ -902,43 +902,43 @@ begin
   apply biimp_refl, refl
 end
 
-@[refl] def equiv_preformulae_refl (T : set formula) {l} (f : preformula l) : 
+@[refl] def equiv_preformulae_refl (T : set (formula L)) {l} (f : preformula L l) : 
   equiv_preformulae T f f :=
 λxs, biimp_refl T (apps_rel f xs)
 
 /- model theory -/
 
 /- an L-structure is a type S with interpretations of the functions and relations on S -/
-parameter (L)
+variable (L)
 structure Structure :=
 (carrier : Type u) 
 (fun_map : ∀{n}, L.functions n → dvector carrier n → carrier)
 (rel_map : ∀{n}, L.relations n → dvector carrier n → Prop) 
-parameter {L}
+variable {L}
 instance has_coe_Structure : has_coe_to_sort (@_root_.fol.Structure L) :=
 ⟨Type u, Structure.carrier⟩
 
 /- realization of terms -/
-@[simp] def realize_term {S : Structure} (v : ℕ → S) : 
-  ∀{l} (t : preterm l) (xs : dvector S l), S.carrier
+@[simp] def realize_term {S : Structure L} (v : ℕ → S) : 
+  ∀{l} (t : preterm L l) (xs : dvector S l), S.carrier
 | _ &k          xs := v k
 | _ (func f)    xs := S.fun_map f xs
 | _ (app t₁ t₂) xs := realize_term t₁ $ realize_term t₂ ([])::xs
 
-lemma realize_term_congr {S : Structure} {v v' : ℕ → S} (h : ∀n, v n = v' n) : 
-  ∀{l} (t : preterm l) (xs : dvector S l), realize_term v t xs = realize_term v' t xs
+lemma realize_term_congr {S : Structure L} {v v' : ℕ → S} (h : ∀n, v n = v' n) : 
+  ∀{l} (t : preterm L l) (xs : dvector S l), realize_term v t xs = realize_term v' t xs
 | _ &k          xs := h k
 | _ (func f)    xs := by refl
 | _ (app t₁ t₂) xs := by dsimp; rw [realize_term_congr t₁, realize_term_congr t₂]
 
-lemma realize_term_subst {S : Structure} (v : ℕ → S) : ∀{l} (n : ℕ) (t : preterm l) 
-  (s : term) (xs : dvector S l), realize_term (v[realize_term v (s ↑ n) ([]) // n]) t xs = realize_term v (t[s // n]) xs
+lemma realize_term_subst {S : Structure L} (v : ℕ → S) : ∀{l} (n : ℕ) (t : preterm L l) 
+  (s : term L) (xs : dvector S l), realize_term (v[realize_term v (s ↑ n) ([]) // n]) t xs = realize_term v (t[s // n]) xs
 | _ n &k          s [] := 
   by apply lt_by_cases k n; intro h;[simp [h], {subst h; simp}, simp [h]]
 | _ n (func f)    s xs := by refl
 | _ n (app t₁ t₂) s xs := by dsimp; simp*
 
-lemma realize_term_subst_lift {S : Structure} (v : ℕ → S) (x : S) (m : ℕ) : ∀{l} (t : preterm l)
+lemma realize_term_subst_lift {S : Structure L} (v : ℕ → S) (x : S) (m : ℕ) : ∀{l} (t : preterm L l)
   (xs : dvector S l), realize_term (v [x // m]) (t ↑' 1 # m) xs = realize_term v t xs
 | _ &k          [] := 
   begin 
@@ -950,7 +950,7 @@ lemma realize_term_subst_lift {S : Structure} (v : ℕ → S) (x : S) (m : ℕ) 
 | _ (app t₁ t₂) xs := by simp*
 
 /- realization of formulas -/
-@[simp] def realize_formula {S : Structure} : ∀{l}, (ℕ → S) → preformula l → dvector S l → Prop
+@[simp] def realize_formula {S : Structure L} : ∀{l}, (ℕ → S) → preformula L l → dvector S l → Prop
 | _ v falsum       xs := false
 | _ v (t₁ ≃ t₂)    xs := realize_term v t₁ xs = realize_term v t₂ xs
 | _ v (rel R)      xs := S.rel_map R xs
@@ -958,8 +958,8 @@ lemma realize_term_subst_lift {S : Structure} (v : ℕ → S) (x : S) (m : ℕ) 
 | _ v (f₁ ⟹ f₂)   xs := realize_formula v f₁ xs → realize_formula v f₂ xs
 | _ v (∀' f)       xs := ∀(x : S), realize_formula (v [x // 0]) f xs
 
-lemma realize_formula_congr {S : Structure} : ∀{l} {v v' : ℕ → S} (h : ∀n, v n = v' n) 
-  (f : preformula l) (xs : dvector S l), realize_formula v f xs ↔ realize_formula v' f xs
+lemma realize_formula_congr {S : Structure L} : ∀{l} {v v' : ℕ → S} (h : ∀n, v n = v' n) 
+  (f : preformula L l) (xs : dvector S l), realize_formula v f xs ↔ realize_formula v' f xs
 | _ v v' h falsum       xs := by refl
 | _ v v' h (t₁ ≃ t₂)    xs := by simp [realize_term_congr h]
 | _ v v' h (rel R)      xs := by refl
@@ -969,8 +969,8 @@ lemma realize_formula_congr {S : Structure} : ∀{l} {v v' : ℕ → S} (h : ∀
   by apply forall_congr; intro x; apply realize_formula_congr; intro n; 
      apply subst_realize_congr h
 
-lemma realize_formula_subst {S : Structure} : ∀{l} (v : ℕ → S) (n : ℕ) (f : preformula l) 
-  (s : term) (xs : dvector S l), realize_formula (v[realize_term v (s ↑ n) ([]) // n]) f xs ↔ realize_formula v (f[s // n]) xs
+lemma realize_formula_subst {S : Structure L} : ∀{l} (v : ℕ → S) (n : ℕ) (f : preformula L l) 
+  (s : term L) (xs : dvector S l), realize_formula (v[realize_term v (s ↑ n) ([]) // n]) f xs ↔ realize_formula v (f[s // n]) xs
 | _ v n falsum       s xs := by refl
 | _ v n (t₁ ≃ t₂)    s xs := by simp [realize_term_subst]
 | _ v n (rel R)      s xs := by refl
@@ -982,12 +982,12 @@ lemma realize_formula_subst {S : Structure} : ∀{l} (v : ℕ → S) (n : ℕ) (
     intro k, rw [subst_realize2_0, ←realize_term_subst_lift v x 0, lift_term_def, lift_term2]
   end
 
-lemma realize_formula_subst0 {S : Structure} {l} (v : ℕ → S) (f : preformula l) (s : term) (xs : dvector S l) :
+lemma realize_formula_subst0 {S : Structure L} {l} (v : ℕ → S) (f : preformula L l) (s : term L) (xs : dvector S l) :
   realize_formula (v[realize_term v s ([]) // 0]) f xs ↔ realize_formula v (f[s // 0]) xs :=
 by have h := realize_formula_subst v 0 f s; simp at h; exact h xs
 
-lemma realize_formula_subst_lift {S : Structure} : ∀{l} (v : ℕ → S) (x : S) (m : ℕ) 
-  (f : preformula l) (xs : dvector S l), realize_formula (v [x // m]) (f ↑' 1 # m) xs = realize_formula v f xs
+lemma realize_formula_subst_lift {S : Structure L} : ∀{l} (v : ℕ → S) (x : S) (m : ℕ) 
+  (f : preformula L l) (xs : dvector S l), realize_formula (v [x // m]) (f ↑' 1 # m) xs = realize_formula v f xs
 | _ v x m falsum       xs := by refl
 | _ v x m (t₁ ≃ t₂)    xs := by simp [realize_term_subst_lift]
 | _ v x m (rel R)      xs := by refl
@@ -1001,49 +1001,49 @@ lemma realize_formula_subst_lift {S : Structure} : ∀{l} (v : ℕ → S) (x : S
 
 /- the following definitions of provability and satisfiability are not exactly how you normally define them, since we define it for formulae instead of sentences. If all the formulae happen to be sentences, then these definitions are equivalent to the normal definitions (the realization of closed terms and sentences are independent of the realizer v). 
  -/
-def all_prf (T T' : set formula) := ∀{{f}}, f ∈ T' → T ⊢ f
+def all_prf (T T' : set (formula L)) := ∀{{f}}, f ∈ T' → T ⊢ f
 infix ` ⊢ `:51 := _root_.fol.all_prf -- input: |- or \vdash
 
-def satisfied_in (S : Structure) (f : formula) := ∀(v : ℕ → S), realize_formula v f ([])
+def satisfied_in (S : Structure L) (f : formula L) := ∀(v : ℕ → S), realize_formula v f ([])
 infix ` ⊨ `:51 := _root_.fol.satisfied_in -- input using \|= or \vDash, but not using \models 
 
-def all_satisfied_in (S : Structure) (T : set formula) := ∀{{f}}, f ∈ T → S ⊨ f
+def all_satisfied_in (S : Structure L) (T : set (formula L)) := ∀{{f}}, f ∈ T → S ⊨ f
 infix ` ⊨ `:51 := _root_.fol.all_satisfied_in -- input using \|= or \vDash, but not using \models 
 
-def satisfied (T : set formula) (f : formula) := 
-∀(S : Structure) (v : ℕ → S), (∀f' ∈ T, realize_formula v (f' : formula) ([])) → 
+def satisfied (T : set (formula L)) (f : formula L) := 
+∀(S : Structure L) (v : ℕ → S), (∀f' ∈ T, realize_formula v (f' : formula L) ([])) → 
   realize_formula v f ([])
 
 infix ` ⊨ `:51 := _root_.fol.satisfied -- input using \|= or \vDash, but not using \models 
 
-def all_satisfied (T T' : set formula) := ∀{{f}}, f ∈ T' → T ⊨ f
+def all_satisfied (T T' : set (formula L)) := ∀{{f}}, f ∈ T' → T ⊨ f
 infix ` ⊨ `:51 := _root_.fol.all_satisfied -- input using \|= or \vDash, but not using \models 
 
-def satisfied_in_trans {S : Structure} {T : set formula} {f : formula} (H' : S ⊨ T) (H : T ⊨ f) :
+def satisfied_in_trans {S : Structure L} {T : set (formula L)} {f : formula L} (H' : S ⊨ T) (H : T ⊨ f) :
   S ⊨ f :=
 λv, H S v $ λf' hf', H' hf' v
 
-def all_satisfied_in_trans  {S : Structure} {T T' : set formula} (H' : S ⊨ T) (H : T ⊨ T') :
+def all_satisfied_in_trans  {S : Structure L} {T T' : set (formula L)} (H' : S ⊨ T) (H : T ⊨ T') :
   S ⊨ T' :=
 λf hf, satisfied_in_trans H' $ H hf
 
-def satisfied_of_mem {T : set formula} {f : formula} (hf : f ∈ T) : T ⊨ f :=
+def satisfied_of_mem {T : set (formula L)} {f : formula L} (hf : f ∈ T) : T ⊨ f :=
 λS v h, h f hf
 
-def all_satisfied_of_subset {T T' : set formula} (h : T' ⊆ T) : T ⊨ T' :=
+def all_satisfied_of_subset {T T' : set (formula L)} (h : T' ⊆ T) : T ⊨ T' :=
 λf hf, satisfied_of_mem $ h hf
 
-def satisfied_trans {T₁ T₂ : set formula} {f : formula} (H' : T₁ ⊨ T₂) (H : T₂ ⊨ f) : T₁ ⊨ f :=
+def satisfied_trans {T₁ T₂ : set (formula L)} {f : formula L} (H' : T₁ ⊨ T₂) (H : T₂ ⊨ f) : T₁ ⊨ f :=
 λS v h, H S v $ λf' hf', H' hf' S v h
 
-def all_satisfied_trans {T₁ T₂ T₃ : set formula} (H' : T₁ ⊨ T₂) (H : T₂ ⊨ T₃) : T₁ ⊨ T₃ :=
+def all_satisfied_trans {T₁ T₂ T₃ : set (formula L)} (H' : T₁ ⊨ T₂) (H : T₂ ⊨ T₃) : T₁ ⊨ T₃ :=
 λf hf, satisfied_trans H' $ H hf
 
-def sweakening {T T' : set formula} (H : T ⊆ T') {f : formula} (HT : T ⊨ f) : T' ⊨ f :=
+def sweakening {T T' : set (formula L)} (H : T ⊆ T') {f : formula L} (HT : T ⊨ f) : T' ⊨ f :=
 λS v h, HT S v $ λf' hf', h f' $ H hf'
 
 /- soundness for a set of formulae -/
-lemma formula_soundness {Γ : set formula} {A : formula} (H : Γ ⊢ A) : Γ ⊨ A :=
+lemma formula_soundness {Γ : set (formula L)} {A : formula L} (H : Γ ⊢ A) : Γ ⊨ A :=
 begin
   intro S, induction H; intros v h,
   { apply h, apply H_h },
@@ -1060,42 +1060,42 @@ begin
 end
 
 /- sentences and theories -/
-inductive term_below (n : ℕ) : ∀{l}, preterm l → Type u
+inductive term_below (n : ℕ) : ∀{l}, preterm L l → Type u
 | b_var' (k) (hk : k < n) : term_below &k
 | b_func {} {l} (f : L.functions l) : term_below (func f)
-| b_app' {l} (t₁ : preterm (l+1)) (t₂ : term) (ht₁ : term_below t₁) (ht₂ : term_below t₂) : 
+| b_app' {l} (t₁ : preterm L (l+1)) (t₂ : term L) (ht₁ : term_below t₁) (ht₂ : term_below t₂) : 
     term_below (app t₁ t₂)
 
 export term_below 
 
-@[reducible, simp] def b_var {n k : ℕ} (hk : k < n) : term_below n &k := b_var' k hk
-@[reducible, simp] def b_app {n l : ℕ} {t₁ : preterm (l+1)} {t₂ : term} (ht₁ : term_below n t₁) 
+@[reducible, simp] def b_var {n k : ℕ} (hk : k < n) : term_below n (&k : term L) := b_var' k hk
+@[reducible, simp] def b_app {n l : ℕ} {t₁ : preterm L (l+1)} {t₂ : term L} (ht₁ : term_below n t₁) 
   (ht₂ : term_below n t₂) : term_below n (app t₁ t₂) := b_app' t₁ t₂ ht₁ ht₂
 
-lemma lift_term_below {n : ℕ} : ∀{l} {t : preterm l} (ht : term_below n t) (n') {m : ℕ}
+lemma lift_term_below {n : ℕ} : ∀{l} {t : preterm L l} (ht : term_below n t) (n') {m : ℕ}
   (h : n ≤ m), t ↑' n' # m = t
 | _ _ (b_var' k hk)          n' m h := 
   have h' : ¬(m ≤ k), from not_le_of_lt (lt_of_lt_of_le hk h), by simp [h']
 | _ _ (b_func f)             n' m h := by refl
 | _ _ (b_app' t₁ t₂ ht₁ ht₂) n' m h := by simp [lift_term_below ht₁ n' h, lift_term_below ht₂ n' h]
 
-@[simp] def realize_term_below {S : Structure} {n} (v : dvector S n) : 
-  ∀{l} {t : preterm l} (ht : term_below n t) (xs : dvector S l), S.carrier
+@[simp] def realize_term_below {S : Structure L} {n} (v : dvector S n) : 
+  ∀{l} {t : preterm L l} (ht : term_below n t) (xs : dvector S l), S.carrier
 | _ _ (b_var' k hk)          xs := v.nth k hk
 | _ _ (b_func f)             xs := S.fun_map f xs
 | _ _ (b_app' t₁ t₂ ht₁ ht₂) xs := realize_term_below ht₁ $ realize_term_below ht₂ ([])::xs
 
-lemma realize_term_below_eq {S : Structure} {n} {v₁ : dvector S n} {v₂ : ℕ → S}
-  (hv : ∀k (hk : k < n), v₁.nth k hk = v₂ k) : ∀{l} {t : preterm l} (ht : term_below n t)
+lemma realize_term_below_eq {S : Structure L} {n} {v₁ : dvector S n} {v₂ : ℕ → S}
+  (hv : ∀k (hk : k < n), v₁.nth k hk = v₂ k) : ∀{l} {t : preterm L l} (ht : term_below n t)
   (xs : dvector S l), realize_term_below v₁ ht xs = realize_term v₂ t xs
 | _ _ (b_var' k hk)          xs := hv k hk
 | _ _ (b_func f)             xs := by refl
 | _ _ (b_app' t₁ t₂ ht₁ ht₂) xs := by simp [realize_term_below_eq ht₁, realize_term_below_eq ht₂]
 
-lemma realize_term_below_irrel' {S : Structure} {n₀ n n'} {v₁ : dvector S n} 
+lemma realize_term_below_irrel' {S : Structure L} {n₀ n n'} {v₁ : dvector S n} 
   {v₂ : dvector S n'} 
   (h : ∀m (hn₀ : m < n₀) (hn : m < n) (hn' : m < n'), v₁.nth m hn = v₂.nth m hn')
-  {l} {t : preterm l} (ht : term_below n t) (ht' : term_below n' t) 
+  {l} {t : preterm L l} (ht : term_below n t) (ht' : term_below n' t) 
   (ht0 : term_below n₀ t) (xs : dvector S l) : 
   realize_term_below v₁ ht xs = realize_term_below v₂ ht' xs :=
 begin
@@ -1105,14 +1105,14 @@ begin
   { simp [ht0_ih_ht₁ ht_ht₁ ht'_ht₁, ht0_ih_ht₂ ht_ht₂ ht'_ht₂] }
 end
 
-lemma realize_term_below_irrel {S : Structure} {n n'} {v₁ : dvector S n} 
+lemma realize_term_below_irrel {S : Structure L} {n n'} {v₁ : dvector S n} 
   {v₂ : dvector S n'} 
-  {l} {t : preterm l} (ht : term_below n t) (ht' : term_below n' t) 
+  {l} {t : preterm L l} (ht : term_below n t) (ht' : term_below n' t) 
   (ht0 : term_below 0 t) (xs : dvector S l) :
   realize_term_below v₁ ht xs = realize_term_below v₂ ht' xs :=
 realize_term_below_irrel' (by intros m hm; exfalso; apply not_lt_zero m hm) ht ht' ht0 xs
 
-@[simp] def term_below_lift {n} (n' m) : ∀{l} {t : preterm l} (ht : term_below n t), 
+@[simp] def term_below_lift {n} (n' m) : ∀{l} {t : preterm L l} (ht : term_below n t), 
   term_below (n + n') (t ↑' n' # m)
 | _ _ (b_var' k hk)          := 
   begin 
@@ -1123,11 +1123,11 @@ realize_term_below_irrel' (by intros m hm; exfalso; apply not_lt_zero m hm) ht h
 | _ _ (b_func f)             := b_func f
 | _ _ (b_app' t₁ t₂ ht₁ ht₂) := b_app (term_below_lift ht₁) (term_below_lift ht₂)
 
-def term_below_lift0 {n m l} {t : preterm l} (ht : term_below 0 t) : term_below n (t ↑' n # m) :=
+def term_below_lift0 {n m l} {t : preterm L l} (ht : term_below 0 t) : term_below n (t ↑' n # m) :=
 by have := term_below_lift n m ht; rw [zero_add] at this; exact this
 
-def term_below_subst {n n'} : ∀{l} {t : preterm l} (ht : term_below (n+n'+1) t) 
-  {s : term} (hs : term_below n' s), term_below (n+n') (t[s // n])
+def term_below_subst {n n'} : ∀{l} {t : preterm L l} (ht : term_below (n+n'+1) t) 
+  {s : term L} (hs : term_below n' s), term_below (n+n') (t[s // n])
 | _ _ (b_var' k hk)          s hs := 
   begin
     apply lt_by_cases n k; intro h; simp [h],
@@ -1138,69 +1138,70 @@ def term_below_subst {n n'} : ∀{l} {t : preterm l} (ht : term_below (n+n'+1) t
 | _ _ (b_func f)             s hs := b_func f
 | _ _ (b_app' t₁ t₂ ht₁ ht₂) s hs := b_app (term_below_subst ht₁ hs) (term_below_subst ht₂ hs)
 
-def term_below_subst_closed {n l} {t : preterm l} (hf : term_below (n+1) t) 
-  {s : term} (hs : term_below 0 s) : term_below n (t[s // n]) :=
+def term_below_subst_closed {n l} {t : preterm L l} (hf : term_below (n+1) t) 
+  {s : term L} (hs : term_below 0 s) : term_below n (t[s // n]) :=
 term_below_subst (by exact hf) hs
 
-instance subsingleton_term_below (n : ℕ) {l} (t : preterm l) : subsingleton (term_below n t) :=
+instance subsingleton_term_below (n : ℕ) {l} (t : preterm L l) : subsingleton (term_below n t) :=
 begin
   constructor, intros h h', induction h generalizing h'; cases h'; try {refl}; congr,
   apply h_ih_ht₁, apply h_ih_ht₂
 end
 
-def term_below_of_le : ∀ {l} {t : preterm l} {n m : ℕ}, n ≤ m → term_below n t → term_below m t
+def term_below_of_le : ∀ {l} {t : preterm L l} {n m : ℕ}, n ≤ m → term_below n t → term_below m t
 | _ _ n m h (b_var' k hk)          := b_var $ lt_of_lt_of_le hk h
 | _ _ n m h (b_func f)             := b_func f
 | _ _ n m h (b_app' t₁ t₂ ht₁ ht₂) := b_app (term_below_of_le h ht₁) (term_below_of_le h ht₂)
 
-def term_below_of_zero {l} {t : preterm l} {n : ℕ} (ht : term_below 0 t) : term_below n t :=
+def term_below_of_zero {l} {t : preterm L l} {n : ℕ} (ht : term_below 0 t) : term_below n t :=
 term_below_of_le n.zero_le ht
 
-parameter (L)
-def bounded_preterm (n l) := Σ(t : preterm l), term_below n t
-def bounded_term    (n)   := Σ(t : term),      term_below n t
-def closed_preterm  (l)   := Σ(t : preterm l), term_below 0 t
-def closed_term           := Σ(t : term),      term_below 0 t
-parameter {L}
+variable (L)
+def bounded_preterm (n l) := Σ(t : preterm L l), term_below n t
+def bounded_term    (n)   := Σ(t : term L),      term_below n t
+def closed_preterm  (l)   := Σ(t : preterm L l), term_below 0 t
+def closed_term           := Σ(t : term L),      term_below 0 t
+variable {L}
 
-def closed_term.eq {n l} {t₁ t₂ : bounded_preterm n l} (h : t₁.fst = t₂.fst) : t₁ = t₂ :=
+def closed_term.eq {n l} {t₁ t₂ : bounded_preterm L n l} (h : t₁.fst = t₂.fst) : t₁ = t₂ :=
 sigma.eq h (subsingleton.elim _ _)
 
--- @[reducible] def closed_term.fst : closed_term → term := sigma.fst
+-- @[reducible] def closed_term.fst : closed_term L → term := sigma.fst
 
-def bounded_term_of_closed_term {l n} (t : closed_preterm l) : bounded_preterm n l :=
+def bounded_term_of_closed_term {l n} (t : closed_preterm L l) : bounded_preterm L n l :=
 ⟨t.fst, term_below_of_zero t.snd⟩
 
-def bounded_term_lift1 {l n} (t : bounded_preterm n l) : bounded_preterm (n+1) l :=
+def bounded_term_lift1 {l n} (t : bounded_preterm L n l) : bounded_preterm L (n+1) l :=
 ⟨t.fst, term_below_of_le (nat.le_add_right n 1) t.snd⟩
 
-def bd_var {n} (k : fin n) : bounded_term n := ⟨&k.val, b_var k.is_lt⟩
+def bd_var {n} (k : fin n) : bounded_term L n := ⟨&k.val, b_var k.is_lt⟩
 prefix `&`:max := _root_.fol.bd_var
-def bd_func {n l} (f : L.functions l) : bounded_preterm n l := ⟨func f, b_func f⟩
-def bd_const {n} (c : L.constants) : bounded_term n := bd_func c
-def bd_app {n l} (t₁ : bounded_preterm n (l+1)) (t₂ : bounded_term n) : bounded_preterm n l := 
+def bd_func {n l} (f : L.functions l) : bounded_preterm L n l := ⟨func f, b_func f⟩
+def bd_const {n} (c : L.constants) : bounded_term L n := bd_func c
+def bd_app {n l} (t₁ : bounded_preterm L n (l+1)) (t₂ : bounded_term L n) : bounded_preterm L n l := 
 ⟨app t₁.fst t₂.fst, b_app t₁.snd t₂.snd⟩
-def c_func {l} (f : L.functions l) : closed_preterm l := bd_func f
-def c_const (c : L.constants) : closed_term := c_func c
-def c_app {l} (t₁ : closed_preterm (l+1)) (t₂ : closed_term) : closed_preterm l := bd_app t₁ t₂
+def c_func {l} (f : L.functions l) : closed_preterm L l := bd_func f
+def c_const (c : L.constants) : closed_term L := c_func c
+def c_app {l} (t₁ : closed_preterm L (l+1)) (t₂ : closed_term L) : closed_preterm L l := bd_app t₁ t₂
 
-@[simp] def bd_apps {n} : ∀{l}, bounded_preterm n l → dvector (bounded_term n) l → bounded_term n
+@[simp] def bd_apps {n} : ∀{l}, bounded_preterm L n l → dvector (bounded_term L n) l → 
+  bounded_term L n
 | _ t []       := t
 | _ t (t'::ts) := bd_apps (bd_app t t') ts
 
-def c_apps {l} : closed_preterm l → dvector closed_term l → closed_term :=
+def c_apps {l} : closed_preterm L l → dvector (closed_term L) l → closed_term L :=
 bd_apps
 
 def bounded_term_of_function {l n} (f : L.functions l) : 
-  arity (bounded_term n) (bounded_term n) l :=
+  arity (bounded_term L n) (bounded_term L n) l :=
 arity.of_dvector_map $ bd_apps (bd_func f)
 
-def bounded_preterm.rec {n} {C : Πl, bounded_preterm n l → Sort v}
+def bounded_preterm.rec {n} {C : Πl, bounded_preterm L n l → Sort v}
   (Hvar : Πk, C 0 &k)
   (Hfun : Π {l} (f : L.functions l), C l (bd_func f))
-  (Happ : Π {l} {t : bounded_preterm n (l+1)} {s : bounded_term n} (ih_t : C (l+1) t) 
+  (Happ : Π {l} {t : bounded_preterm L n (l+1)} {s : bounded_term L n} (ih_t : C (l+1) t) 
     (ih_s : C 0 s), C l (bd_app t s))
-  {{l : ℕ}} (f : bounded_preterm n l) : C l f :=
+  {{l : ℕ}} (f : bounded_preterm L n l) : C l f :=
 begin
   induction f with f hf, induction hf,
   { exact Hvar ⟨hf_k, hf_hk⟩ },
@@ -1208,66 +1209,66 @@ begin
   { exact @Happ _ ⟨hf_t₁, hf_ht₁⟩ ⟨hf_t₂, hf_ht₂⟩ hf_ih_ht₁ hf_ih_ht₂ }
 end
 
-def realize_bounded_term {S : Structure} {n} (v : dvector S n)
-  {l} (t : bounded_preterm n l) (xs : dvector S l) : S :=
+def realize_bounded_term {S : Structure L} {n} (v : dvector S n)
+  {l} (t : bounded_preterm L n l) (xs : dvector S l) : S :=
 realize_term_below v t.snd xs
 
-@[reducible] def realize_closed_term (S : Structure) (t : closed_term) : S :=
+@[reducible] def realize_closed_term (S : Structure L) (t : closed_term L) : S :=
 realize_bounded_term ([]) t ([])
 
-@[simp] lemma realize_bounded_term_bd_app {S : Structure}
-  {n l} (t : bounded_preterm n (l+1)) (s : bounded_term n) (xs : dvector S n) 
+@[simp] lemma realize_bounded_term_bd_app {S : Structure L}
+  {n l} (t : bounded_preterm L n (l+1)) (s : bounded_term L n) (xs : dvector S n) 
   (xs' : dvector S l) :
   realize_bounded_term xs (bd_app t s) xs' = 
   realize_bounded_term xs t (realize_bounded_term xs s ([])::xs') :=
 by refl
 
-@[simp] lemma realize_closed_term_bd_apps {S : Structure}
-  {l} (t : closed_preterm l) (ts : dvector closed_term l) :
+@[simp] lemma realize_closed_term_bd_apps {S : Structure L}
+  {l} (t : closed_preterm L l) (ts : dvector (closed_term L) l) :
   realize_closed_term S (bd_apps t ts) = 
   realize_bounded_term ([]) t (ts.map (λt', realize_bounded_term ([]) t' ([]))) :=
 begin
   induction ts generalizing t, refl, apply ts_ih (bd_app t ts_x)
 end
 
-def lift_bounded_term_at {n' l} (t : bounded_preterm n' l) (n m : ℕ) : 
-  bounded_preterm (n'+n) l :=
+def lift_bounded_term_at {n' l} (t : bounded_preterm L n' l) (n m : ℕ) : 
+  bounded_preterm L (n'+n) l :=
 ⟨t.fst ↑' n # m, term_below_lift n m t.snd⟩
 notation t ` ↑' `:90 n ` # `:90 m:90 := _root_.fol.lift_bounded_term_at t n m -- input ↑ with \u or \upa
 
-@[reducible] def lift_bounded_term {n' l} (t : bounded_preterm n' l) (n : ℕ) : 
-  bounded_preterm (n'+n) l := 
+@[reducible] def lift_bounded_term {n' l} (t : bounded_preterm L n' l) (n : ℕ) : 
+  bounded_preterm L (n'+n) l := 
 t ↑' n # 0
 infix ` ↑ `:100 := _root_.fol.lift_bounded_term -- input ↑' with \u or \upa
-@[reducible, simp] def lift_bounded_term1 {n' l} (t : bounded_preterm n' l) : 
-  bounded_preterm (n'+1) l := 
+@[reducible, simp] def lift_bounded_term1 {n' l} (t : bounded_preterm L n' l) : 
+  bounded_preterm L (n'+1) l := 
 t ↑ 1
 
-def substmax_bounded_term {n l} (t : bounded_preterm (n+1) l) (s : closed_term) :
-  bounded_preterm n l :=
+def substmax_bounded_term {n l} (t : bounded_preterm L (n+1) l) (s : closed_term L) :
+  bounded_preterm L n l :=
 ⟨t.fst[s.fst // n], term_below_subst_closed t.snd s.snd⟩
 
-def substmax_var_lt {n} (k : fin (n+1)) (s : closed_term) (h : k.1 < n) :
+def substmax_var_lt {n} (k : fin (n+1)) (s : closed_term L) (h : k.1 < n) :
   substmax_bounded_term &k s = &⟨k.1, h⟩ :=
 begin
   apply closed_term.eq, simp [substmax_bounded_term, bd_var, h]
 end
 
-def substmax_var_eq {n} (k : fin (n+1)) (s : closed_term) (h : k.1 = n) :
+def substmax_var_eq {n} (k : fin (n+1)) (s : closed_term L) (h : k.1 = n) :
   substmax_bounded_term &k s = bounded_term_of_closed_term s :=
 begin
   apply closed_term.eq, simp [substmax_bounded_term, bd_var],
   simp [h], dsimp only [lift_term], rw [lift_term_below s.2 _ (le_refl _)], refl
 end
 
--- lemma substmax_bounded_term_bd_apps {n l} (t : bounded_preterm (n+1) l) 
---   (s : closed_term) (ts : dvector (bounded_term (n+1)) l) :
+-- lemma substmax_bounded_term_bd_apps {n l} (t : bounded_preterm L (n+1) l) 
+--   (s : closed_term L) (ts : dvector (bounded_term (n+1)) l) :
 --   substmax_bounded_term (bd_apps t ts) s = 
 --   bd_apps (substmax_bounded_term t s) (ts.map $ λt', substmax_bounded_term t' s) :=
 -- sorry
 
-lemma realize_bounded_term_bd_apps {S : Structure}
-  {n l} (xs : dvector S n) (t : bounded_preterm n l) (ts : dvector (bounded_term n) l) :
+lemma realize_bounded_term_bd_apps {S : Structure L}
+  {n l} (xs : dvector S n) (t : bounded_preterm L n l) (ts : dvector (bounded_term L n) l) :
   realize_bounded_term xs (bd_apps t ts) ([]) =
   realize_bounded_term xs t (ts.map (λt, realize_bounded_term xs t ([]))) :=
 begin
@@ -1276,55 +1277,55 @@ end
 
 /- this is the same as realize_term_below, we should probably have a common generalization of this definition -/
 -- @[simp] def substitute_term_below {n n'} (v : dvector (bounded_term n') n) : 
---   ∀{l} {t : preterm l} (ht : term_below n t), bounded_preterm n' l
+--   ∀{l} {t : preterm L l} (ht : term_below n t), bounded_preterm L n' l
 -- | _ _ (b_var' k hk)          := v.nth k hk
 -- | _ _ (b_func f)             := bd_func f
 -- | _ _ (b_app' t₁ t₂ ht₁ ht₂) := bd_app (substitute_term_below ht₁) $ substitute_term_below ht₂
 
--- def substitute_bounded_term {n n' l} (t : bounded_preterm n l) 
---   (v : dvector (bounded_term n') n) : bounded_preterm n' l :=
+-- def substitute_bounded_term {n n' l} (t : bounded_preterm L n l) 
+--   (v : dvector (bounded_term n') n) : bounded_preterm L n' l :=
 -- substitute_term_below v t.snd
 
-inductive formula_below : ∀{l}, ℕ → preformula l → Type u
+inductive formula_below : ∀{l}, ℕ → preformula L l → Type u
 | b_falsum {n} : formula_below n falsum
 | b_equal' {n} (t₁ t₂) (ht₁ : term_below n t₁) (ht₂ : term_below n t₂) : 
     formula_below n (t₁ ≃ t₂)
 | b_rel {n l} (R : L.relations l) : formula_below n (rel R)
-| b_apprel' {n l} (f : preformula (l+1)) (t) (hf : formula_below n f) 
+| b_apprel' {n l} (f : preformula L (l+1)) (t) (hf : formula_below n f) 
     (ht : term_below n t) : formula_below n (apprel f t)
-| b_imp' {n} (f₁ f₂ : formula) (hf₁ : formula_below n f₁) (hf₂ : formula_below n f₂) :
+| b_imp' {n} (f₁ f₂ : formula L) (hf₁ : formula_below n f₁) (hf₂ : formula_below n f₂) :
     formula_below n (f₁ ⟹ f₂)
-| b_all' {n} (f : formula) (hf : formula_below (n+1) f) : formula_below n (∀' f)
+| b_all' {n} (f : formula L) (hf : formula_below (n+1) f) : formula_below n (∀' f)
 export formula_below
 
-@[reducible, simp] def b_equal {n : ℕ} {t₁ t₂ : term} (ht₁ : term_below n t₁) 
+@[reducible, simp] def b_equal {n : ℕ} {t₁ t₂ : term L} (ht₁ : term_below n t₁) 
   (ht₂ : term_below n t₂) : formula_below n (t₁ ≃ t₂) := 
 b_equal' t₁ t₂ ht₁ ht₂
 
-@[reducible, simp] def b_apprel {n l : ℕ} {f : preformula (l+1)} {t : term} 
+@[reducible, simp] def b_apprel {n l : ℕ} {f : preformula L (l+1)} {t : term L} 
   (hf : formula_below n f) (ht : term_below n t) : formula_below n (apprel f t) := 
 b_apprel' f t hf ht
 
-@[reducible, simp] def b_imp {n : ℕ} {f g : formula} (hf : formula_below n f) 
+@[reducible, simp] def b_imp {n : ℕ} {f g : formula L} (hf : formula_below n f) 
   (hg : formula_below n g) : formula_below n (f ⟹ g) := 
 b_imp' f g hf hg
 
-@[reducible, simp] def b_all {n : ℕ} {f : formula} (hf : formula_below (n+1) f) : 
+@[reducible, simp] def b_all {n : ℕ} {f : formula L} (hf : formula_below (n+1) f) : 
   formula_below n (∀' f) := 
 b_all' f hf
 
-def b_not {n : ℕ} {f : formula} (hf : formula_below n f)  : formula_below n (∼f) := 
+def b_not {n : ℕ} {f : formula L} (hf : formula_below n f)  : formula_below n (∼f) := 
 b_imp hf b_falsum
 
-def b_and {n : ℕ} {f g : formula} (hf : formula_below n f) (hg : formula_below n g) : 
+def b_and {n : ℕ} {f g : formula L} (hf : formula_below n f) (hg : formula_below n g) : 
   formula_below n (f ⊓ g) :=
 b_not (b_imp hf (b_not hg))
 
-def b_biimp {n : ℕ} {f g : formula} (hf : formula_below n f) (hg : formula_below n g) : 
+def b_biimp {n : ℕ} {f g : formula L} (hf : formula_below n f) (hg : formula_below n g) : 
   formula_below n (f ⇔ g) :=
 b_and (b_imp hf hg) (b_imp hg hf)
 
-lemma lift_formula_below : ∀{n l} {f : preformula l} (hf : formula_below n f) (n') 
+lemma lift_formula_below : ∀{n l} {f : preformula L l} (hf : formula_below n f) (n') 
   {m : ℕ} (h : n ≤ m), f ↑' n' # m = f
 | n _ _ b_falsum                 n' m h := by refl
 | n _ _ (b_equal' t₁ t₂ ht₁ ht₂) n' m h := 
@@ -1336,8 +1337,8 @@ lemma lift_formula_below : ∀{n l} {f : preformula l} (hf : formula_below n f) 
   by simp [lift_formula_below hf₁ n' h, lift_formula_below hf₂ n' h]
 | n _ _ (b_all' f hf)            n' m h := by simp [lift_formula_below hf n' (add_le_add_right h 1)]
 
-@[simp] def realize_formula_below {S : Structure} : ∀{n} (v : dvector S n)
-  {l} {f : preformula l} (hf : formula_below n f) (xs : dvector S l), Prop
+@[simp] def realize_formula_below {S : Structure L} : ∀{n} (v : dvector S n)
+  {l} {f : preformula L l} (hf : formula_below n f) (xs : dvector S l), Prop
 | n v _ _ b_falsum                 xs := false
 | n v _ _ (b_equal' t₁ t₂ ht₁ ht₂) xs := realize_term_below v ht₁ xs = realize_term_below v ht₂ xs
 | n v _ _ (b_rel R)                xs := S.rel_map R xs
@@ -1347,8 +1348,8 @@ lemma lift_formula_below : ∀{n l} {f : preformula l} (hf : formula_below n f) 
   realize_formula_below v hf₁ xs → realize_formula_below v hf₂ xs
 | n v _ _ (b_all' f hf)            xs := ∀(x : S), realize_formula_below (x::v) hf xs
 
-lemma realize_formula_below_eq {S : Structure} : ∀{n} {v₁ : dvector S n} {v₂ : ℕ → S} 
-  (hv : ∀k (hk : k < n), v₁.nth k hk = v₂ k) {l} {f : preformula l} (hf : formula_below n f)
+lemma realize_formula_below_eq {S : Structure L} : ∀{n} {v₁ : dvector S n} {v₂ : ℕ → S} 
+  (hv : ∀k (hk : k < n), v₁.nth k hk = v₂ k) {l} {f : preformula L l} (hf : formula_below n f)
   (xs : dvector S l), realize_formula_below v₁ hf xs ↔ realize_formula v₂ f xs
 | n v₁ v₂ hv _ _ b_falsum                 xs := by refl
 | n v₁ v₂ hv _ _ (b_equal' t₁ t₂ ht₁ ht₂) xs := 
@@ -1364,7 +1365,7 @@ lemma realize_formula_below_eq {S : Structure} : ∀{n} {v₁ : dvector S n} {v�
     apply subst_fin_realize_eq hv
   end
 
-def formula_below_lift : ∀{n} (n' m) {l} {f : preformula l} (hf : formula_below n f), 
+def formula_below_lift : ∀{n} (n' m) {l} {f : preformula L l} (hf : formula_below n f), 
   formula_below (n + n') (f ↑' n' # m)
 | n n' m _ _ b_falsum                 := b_falsum
 | n n' m _ _ (b_equal' t₁ t₂ ht₁ ht₂) := 
@@ -1380,8 +1381,8 @@ def formula_below_lift : ∀{n} (n' m) {l} {f : preformula l} (hf : formula_belo
       simp only [add_comm, add_left_comm, eq_self_iff_true]
   end
 
-def formula_below_subst : ∀{n n' l} {f : preformula l} (hf : formula_below (n+n'+1) f) 
-  {s : term} (hs : term_below n' s), formula_below (n+n') (f[s // n])
+def formula_below_subst : ∀{n n' l} {f : preformula L l} (hf : formula_below (n+n'+1) f) 
+  {s : term L} (hs : term_below n' s), formula_below (n+n') (f[s // n])
 | n n' _ _ b_falsum                 s hs := b_falsum
 | n n' _ _ (b_equal' t₁ t₂ ht₁ ht₂) s hs := 
   b_equal (term_below_subst ht₁ hs) (term_below_subst ht₂ hs)
@@ -1396,30 +1397,30 @@ def formula_below_subst : ∀{n n' l} {f : preformula l} (hf : formula_below (n+
       simp only [add_comm, add_left_comm],
   end
 
-def formula_below_subst0 {n l} {f : preformula l} (hf : formula_below (n+1) f) 
-  {s : term} (hs : term_below n s) : formula_below n (f[s // 0]) :=
+def formula_below_subst0 {n l} {f : preformula L l} (hf : formula_below (n+1) f) 
+  {s : term L} (hs : term_below n s) : formula_below n (f[s // 0]) :=
 by rw [←zero_add (n+1)] at hf; have := formula_below_subst hf hs; simpa only [zero_add]
 
-def formula_below_subst_closed {n l} {f : preformula l} (hf : formula_below (n+1) f) 
-  {s : term} (hs : term_below 0 s) : formula_below n (f[s // n]) :=
+def formula_below_subst_closed {n l} {f : preformula L l} (hf : formula_below (n+1) f) 
+  {s : term L} (hs : term_below 0 s) : formula_below n (f[s // n]) :=
 formula_below_subst (by exact hf) hs
 
-instance subsingleton_formula_below (n : ℕ) {l} (f : preformula l) : 
+instance subsingleton_formula_below (n : ℕ) {l} (f : preformula L l) : 
   subsingleton (formula_below n f) :=
 begin
   constructor, intros h h', induction h generalizing h'; cases h'; try {refl}; congr,
   apply h_ih, apply h_ih_hf₁, apply h_ih_hf₂, apply h_ih
 end
 
-lemma realize_formula_below_congr {S : Structure} {n} {v₁ v₂ : dvector S n} 
-  (hv : v₁ = v₂) {l} {f : preformula l} {f' : preformula l} (h : f = f') (hf : formula_below n f)(hf' : formula_below n f') : realize_formula_below v₁ hf = realize_formula_below v₂ hf' :=
+lemma realize_formula_below_congr {S : Structure L} {n} {v₁ v₂ : dvector S n} 
+  (hv : v₁ = v₂) {l} {f : preformula L l} {f' : preformula L l} (h : f = f') (hf : formula_below n f)(hf' : formula_below n f') : realize_formula_below v₁ hf = realize_formula_below v₂ hf' :=
 by subst hv; subst h; congr
 
 set_option trace.check true
-lemma realize_formula_below_irrel' {S : Structure} {n₀ n n'} {v₁ : dvector S n} 
+lemma realize_formula_below_irrel' {S : Structure L} {n₀ n n'} {v₁ : dvector S n} 
   {v₂ : dvector S n'} 
   (h : ∀m (hn₀ : m < n₀) (hn : m < n) (hn' : m < n'), v₁.nth m hn = v₂.nth m hn')
-  {l} {f : preformula l} (hf : formula_below n f) (hf' : formula_below n' f) 
+  {l} {f : preformula L l} (hf : formula_below n f) (hf' : formula_below n' f) 
   (hf0 : formula_below n₀ f) (xs : dvector S l) : 
   realize_formula_below v₁ hf xs ↔ realize_formula_below v₂ hf' xs :=
 begin
@@ -1434,12 +1435,12 @@ begin
     cases m, refl, apply h m (lt_of_succ_lt_succ hn₀) }
 end
 
-lemma realize_formula_below_irrel {S : Structure} {n n'} {v₁ : dvector S n} {v₂ : dvector S n'} 
-  {l} {f : preformula l} (hf : formula_below n f) (hf' : formula_below n' f) 
+lemma realize_formula_below_irrel {S : Structure L} {n n'} {v₁ : dvector S n} {v₂ : dvector S n'} 
+  {l} {f : preformula L l} (hf : formula_below n f) (hf' : formula_below n' f) 
   (hf0 : formula_below 0 f) (xs : dvector S l) : realize_formula_below v₁ hf xs ↔ realize_formula_below v₂ hf' xs :=
 realize_formula_below_irrel' (by intros m hm; exfalso; apply not_lt_zero m hm) hf hf' hf0 xs
 
-def formula_below_of_le : ∀ {l} {f : preformula l} {n m : ℕ}, 
+def formula_below_of_le : ∀ {l} {f : preformula L l} {n m : ℕ}, 
   n ≤ m → formula_below n f → formula_below m f
 | _ _ n m h b_falsum                 := b_falsum
 | _ _ n m h (b_equal' t₁ t₂ ht₁ ht₂) := b_equal (term_below_of_le h ht₁) (term_below_of_le h ht₂)
@@ -1449,98 +1450,98 @@ def formula_below_of_le : ∀ {l} {f : preformula l} {n m : ℕ},
   b_imp (formula_below_of_le h hf₁) (formula_below_of_le h hf₂)
 | _ _ n m h (b_all' f hf)            := b_all $ formula_below_of_le (add_le_add_right h 1) hf
 
-def formula_below_of_zero {l} {f : preformula l} {n : ℕ} (hf : formula_below 0 f) : 
+def formula_below_of_zero {l} {f : preformula L l} {n : ℕ} (hf : formula_below 0 f) : 
   formula_below n f :=
 formula_below_of_le n.zero_le hf
 
-parameter (L)
-@[reducible] def bounded_preformula (n l : ℕ) := Σ(f : preformula l), formula_below n f
-@[reducible] def bounded_formula    (n : ℕ)   := Σ(f : formula),      formula_below n f
-@[reducible] def presentence        (l : ℕ)   := Σ(f : preformula l), formula_below 0 f
-@[reducible] def sentence                     := Σ(f : formula),      formula_below 0 f
-parameter {L}
+variable (L)
+@[reducible] def bounded_preformula (n l : ℕ) := Σ(f : preformula L l), formula_below n f
+@[reducible] def bounded_formula    (n : ℕ)   := Σ(f : formula L),      formula_below n f
+@[reducible] def presentence        (l : ℕ)   := Σ(f : preformula L l), formula_below 0 f
+@[reducible] def sentence                     := Σ(f : formula L),      formula_below 0 f
+variable {L}
 
-def sentence.eq {n l} {f₁ f₂ : bounded_preformula n l} (h : f₁.fst = f₂.fst) : f₁ = f₂ :=
+def sentence.eq {n l} {f₁ f₂ : bounded_preformula L n l} (h : f₁.fst = f₂.fst) : f₁ = f₂ :=
 sigma.eq h (subsingleton.elim _ _)
 
--- @[reducible] def sentence.fst : sentence → formula := sigma.fst
+-- @[reducible] def sentence.fst : sentence L → formula L := sigma.fst
 
-def bounded_formula_of_sentence {l n} (f : presentence l) : bounded_preformula n l :=
+def bounded_formula_of_sentence {l n} (f : presentence L l) : bounded_preformula L n l :=
 ⟨f.fst, formula_below_of_zero f.snd⟩
 
-def bounded_formula_lift1 {l n} (f : bounded_preformula n l) : bounded_preformula (n+1) l :=
+def bounded_formula_lift1 {l n} (f : bounded_preformula L n l) : bounded_preformula L (n+1) l :=
 ⟨f.fst, formula_below_of_le (nat.le_add_right n 1) f.snd⟩
 
-def bd_falsum {n} : bounded_formula n := ⟨falsum, b_falsum⟩ 
+def bd_falsum {n} : bounded_formula L n := ⟨falsum, b_falsum⟩ 
 notation `⊥` := _root_.fol.bd_falsum -- input: \bot
-@[reducible] def bd_equal {n} (t₁ t₂ : bounded_term n) : bounded_formula n := 
+@[reducible] def bd_equal {n} (t₁ t₂ : bounded_term L n) : bounded_formula L n := 
 ⟨t₁.fst ≃ t₂.fst, b_equal t₁.snd t₂.snd⟩
 infix ` ≃ `:88 := _root_.fol.bd_equal -- input \~- or \simeq
-def bd_rel {n l} (r : L.relations l) : bounded_preformula n l := ⟨rel r, b_rel r⟩
-def bd_apprel {n l} (f : bounded_preformula n (l+1)) (t : bounded_term n) : 
-  bounded_preformula n l :=
+def bd_rel {n l} (r : L.relations l) : bounded_preformula L n l := ⟨rel r, b_rel r⟩
+def bd_apprel {n l} (f : bounded_preformula L n (l+1)) (t : bounded_term L n) : 
+  bounded_preformula L n l :=
 ⟨apprel f.fst t.fst, b_apprel f.snd t.snd⟩
-def bd_imp {n} (f₁ f₂ : bounded_formula n) : bounded_formula n := 
+def bd_imp {n} (f₁ f₂ : bounded_formula L n) : bounded_formula L n := 
 ⟨f₁.fst ⟹ f₂.fst, b_imp f₁.snd f₂.snd⟩  
 infix ` ⟹ `:62 := _root_.fol.bd_imp -- input \==>
-def bd_not {n} (f : bounded_formula n) : bounded_formula n := ⟨∼ f.fst, b_not f.snd⟩
+def bd_not {n} (f : bounded_formula L n) : bounded_formula L n := ⟨∼ f.fst, b_not f.snd⟩
 prefix `∼`:max := _root_.fol.bd_not -- input \~, the ASCII character ~ has too low precedence
-def bd_and {n} (f₁ f₂ : bounded_formula n) : bounded_formula n := ∼(f₁ ⟹ ∼f₂)
+def bd_and {n} (f₁ f₂ : bounded_formula L n) : bounded_formula L n := ∼(f₁ ⟹ ∼f₂)
 infixr ` ⊓ ` := _root_.fol.bd_and -- input: \sqcap
-def bd_or {n} (f₁ f₂ : bounded_formula n) : bounded_formula n := ∼f₁ ⟹ f₂
+def bd_or {n} (f₁ f₂ : bounded_formula L n) : bounded_formula L n := ∼f₁ ⟹ f₂
 infixr ` ⊔ ` := _root_.fol.bd_or -- input: \sqcup
-def bd_biimp {n} (f₁ f₂ : bounded_formula n) : bounded_formula n := (f₁ ⟹ f₂) ⊓ (f₂ ⟹ f₁)
+def bd_biimp {n} (f₁ f₂ : bounded_formula L n) : bounded_formula L n := (f₁ ⟹ f₂) ⊓ (f₂ ⟹ f₁)
 infix ` ⇔ `:61 := _root_.fol.bd_biimp -- input \<=>
-def bd_all {n} (f : bounded_formula (n+1)) : bounded_formula n := ⟨∀' f.fst, b_all f.snd⟩
+def bd_all {n} (f : bounded_formula L (n+1)) : bounded_formula L n := ⟨∀' f.fst, b_all f.snd⟩
 prefix `∀'`:110 := _root_.fol.bd_all
-def bd_ex {n} (f : bounded_formula (n+1)) : bounded_formula n := 
+def bd_ex {n} (f : bounded_formula L (n+1)) : bounded_formula L n := 
 ∼ (∀' (∼ f))
 prefix `∃'`:110 := _root_.fol.bd_ex
 
-def s_falsum : sentence := ⊥
+def s_falsum : sentence L := ⊥
 --notation `⊥` := _root_.fol.s_falsum -- input: \bot
-def s_equal (t₁ t₂ : closed_term) : sentence := t₁ ≃ t₂
+def s_equal (t₁ t₂ : closed_term L) : sentence L := t₁ ≃ t₂
 --infix ` ≃ `:88 := _root_.fol.s_equal -- input \~- or \simeq
-def s_rel {l} (r : L.relations l) : presentence l := bd_rel r
-def s_apprel {l} (f : presentence (l+1)) (t : closed_term) : presentence l := bd_apprel f t
-def s_imp (f₁ f₂ : sentence) : sentence := f₁ ⟹ f₂
+def s_rel {l} (r : L.relations l) : presentence L l := bd_rel r
+def s_apprel {l} (f : presentence L (l+1)) (t : closed_term L) : presentence L l := bd_apprel f t
+def s_imp (f₁ f₂ : sentence L) : sentence L := f₁ ⟹ f₂
 --infix ` ⟹ `:62 := _root_.fol.s_imp -- input \==>
-def s_not (f : sentence) : sentence := ∼f
+def s_not (f : sentence L) : sentence L := ∼f
 --prefix `∼`:max := _root_.fol.s_not -- input \~, the ASCII character ~ has too low precedence
-def s_and (f₁ f₂ : sentence) : sentence := f₁ ⊓ f₂
+def s_and (f₁ f₂ : sentence L) : sentence L := f₁ ⊓ f₂
 -- infixr ` ⊓ ` := _root_.fol.s_and -- input: \sqcap
-def s_or (f₁ f₂ : sentence) : sentence := f₁ ⊔ f₂
+def s_or (f₁ f₂ : sentence L) : sentence L := f₁ ⊔ f₂
 -- infixr ` ⊔ ` := _root_.fol.s_or -- input: \sqcup
-def s_biimp (f₁ f₂ : sentence) : sentence := f₁ ⇔ f₂
+def s_biimp (f₁ f₂ : sentence L) : sentence L := f₁ ⇔ f₂
 -- infix ` ⇔ `:61 := _root_.fol.s_biimp -- input \<=>
-def s_all (f : bounded_formula 1) : sentence := ∀' f
-def s_ex (f : bounded_formula 1) : sentence := ∃' f
+def s_all (f : bounded_formula L 1) : sentence L := ∀' f
+def s_ex (f : bounded_formula L 1) : sentence L := ∃' f
 
-def bd_apps_rel : ∀{n l} (f : bounded_preformula n l) (ts : dvector (bounded_term n) l),
-  bounded_formula n
+def bd_apps_rel : ∀{n l} (f : bounded_preformula L n l) (ts : dvector (bounded_term L n) l),
+  bounded_formula L n
 | _ _ f []      := f
 | _ _ f (t::ts) := bd_apps_rel (bd_apprel f t) ts
 
-@[simp] lemma bd_apps_rel_zero {n} (f : bounded_formula n) (ts : dvector (bounded_term n) 0) : 
+@[simp] lemma bd_apps_rel_zero {n} (f : bounded_formula L n) (ts : dvector (bounded_term L n) 0) : 
   bd_apps_rel f ts = f :=
 by cases ts; refl
 
-@[simp] def s_apps_rel {l} (f : presentence l) (ts : dvector closed_term l) : sentence :=
+@[simp] def s_apps_rel {l} (f : presentence L l) (ts : dvector (closed_term L) l) : sentence L :=
 bd_apps_rel f ts
 
 def bounded_formula_of_relation {l n} (f : L.relations l) : 
-  arity (bounded_term n) (bounded_formula n) l :=
+  arity (bounded_term L n) (bounded_formula L n) l :=
 arity.of_dvector_map $ bd_apps_rel (bd_rel f)
 
-def bounded_preformula.rec1 {C : Πn l, bounded_preformula (n+1) l → Sort v}
+def bounded_preformula.rec1 {C : Πn l, bounded_preformula L (n+1) l → Sort v}
   (H0 : Π {n}, C n 0 ⊥)
-  (H1 : Π {n} (t₁ t₂ : bounded_term (n+1)), C n 0 (t₁ ≃ t₂))
+  (H1 : Π {n} (t₁ t₂ : bounded_term L (n+1)), C n 0 (t₁ ≃ t₂))
   (H2 : Π {n l : ℕ} (R : L.relations l), C n l (bd_rel R))
-  (H3 : Π {n l : ℕ} (f : bounded_preformula (n+1) (l + 1)) (t : bounded_term (n+1)) 
+  (H3 : Π {n l : ℕ} (f : bounded_preformula L (n+1) (l + 1)) (t : bounded_term L (n+1)) 
     (ih : C n (l + 1) f), C n l (bd_apprel f t))
-  (H4 : Π {n} (f₁ f₂ : bounded_formula (n+1)) (ih₁ : C n 0 f₁) (ih₂ : C n 0 f₂), C n 0 (f₁ ⟹ f₂))
-  (H5 : Π {n} (f : bounded_formula (n+2)) (ih : C (n+1) 0 f), C n 0 (∀' f)) 
-  {{n l : ℕ}} (f : bounded_preformula (n+1) l) : C n l f :=
+  (H4 : Π {n} (f₁ f₂ : bounded_formula L (n+1)) (ih₁ : C n 0 f₁) (ih₂ : C n 0 f₂), C n 0 (f₁ ⟹ f₂))
+  (H5 : Π {n} (f : bounded_formula L (n+2)) (ih : C (n+1) 0 f), C n 0 (∀' f)) 
+  {{n l : ℕ}} (f : bounded_preformula L (n+1) l) : C n l f :=
 begin
   induction f with f hf, induction f generalizing n; cases hf,
   apply H0, 
@@ -1551,15 +1552,15 @@ begin
   exact H5 ⟨f_f, hf_hf⟩ (f_ih _)
 end
 
-def bounded_preformula.rec {C : Πn l, bounded_preformula n l → Sort v}
+def bounded_preformula.rec {C : Πn l, bounded_preformula L n l → Sort v}
   (H0 : Π {n}, C n 0 ⊥)
-  (H1 : Π {n} (t₁ t₂ : bounded_term n), C n 0 (t₁ ≃ t₂))
+  (H1 : Π {n} (t₁ t₂ : bounded_term L n), C n 0 (t₁ ≃ t₂))
   (H2 : Π {n l : ℕ} (R : L.relations l), C n l (bd_rel R))
-  (H3 : Π {n l : ℕ} (f : bounded_preformula n (l + 1)) (t : bounded_term n) (ih : C n (l + 1) f), 
+  (H3 : Π {n l : ℕ} (f : bounded_preformula L n (l + 1)) (t : bounded_term L n) (ih : C n (l + 1) f), 
     C n l (bd_apprel f t))
-  (H4 : Π {n} (f₁ f₂ : bounded_formula n) (ih₁ : C n 0 f₁) (ih₂ : C n 0 f₂), C n 0 (f₁ ⟹ f₂))
-  (H5 : Π {n} (f : bounded_formula (n+1)) (ih : C (n+1) 0 f), C n 0 (∀' f)) 
-  {{n l : ℕ}} (f : bounded_preformula n l) : C n l f :=
+  (H4 : Π {n} (f₁ f₂ : bounded_formula L n) (ih₁ : C n 0 f₁) (ih₂ : C n 0 f₂), C n 0 (f₁ ⟹ f₂))
+  (H5 : Π {n} (f : bounded_formula L (n+1)) (ih : C (n+1) 0 f), C n 0 (∀' f)) 
+  {{n l : ℕ}} (f : bounded_preformula L n l) : C n l f :=
 begin
   induction f with f hf, induction hf,
   apply H0, 
@@ -1570,15 +1571,15 @@ begin
   exact H5 ⟨hf_f, hf_hf⟩ hf_ih
 end
 
-@[elab_as_eliminator] def bounded_formula.rec1 {C : Πn, bounded_formula (n+1) → Sort v}
+@[elab_as_eliminator] def bounded_formula.rec1 {C : Πn, bounded_formula L (n+1) → Sort v}
   (hfalsum : Π {n}, C n ⊥)
-  (hequal : Π {n} (t₁ t₂ : bounded_term (n+1)), C n (t₁ ≃ t₂))
-  (hrel : Π {n l : ℕ} (R : L.relations l) (ts : dvector (bounded_term (n+1)) l), 
+  (hequal : Π {n} (t₁ t₂ : bounded_term L (n+1)), C n (t₁ ≃ t₂))
+  (hrel : Π {n l : ℕ} (R : L.relations l) (ts : dvector (bounded_term L (n+1)) l), 
     C n (bd_apps_rel (bd_rel R) ts))
-  (himp : Π {n} {f₁ f₂ : bounded_formula (n+1)} (ih₁ : C n f₁) (ih₂ : C n f₂), C n (f₁ ⟹ f₂))
-  (hall : Π {n} {f : bounded_formula (n+2)} (ih : C (n+1) f), C n (∀' f)) 
-  {{n : ℕ}} (f : bounded_formula (n+1)) : C n f :=
-have h : ∀{n l} (f : bounded_preformula (n+1) l) (ts : dvector (bounded_term (n+1)) l), 
+  (himp : Π {n} {f₁ f₂ : bounded_formula L (n+1)} (ih₁ : C n f₁) (ih₂ : C n f₂), C n (f₁ ⟹ f₂))
+  (hall : Π {n} {f : bounded_formula L (n+2)} (ih : C (n+1) f), C n (∀' f)) 
+  {{n : ℕ}} (f : bounded_formula L (n+1)) : C n f :=
+have h : ∀{n l} (f : bounded_preformula L (n+1) l) (ts : dvector (bounded_term L (n+1)) l), 
   C n (bd_apps_rel f ts),
 begin
   refine bounded_preformula.rec1 _ _ _ _ _ _; intros; try {rw ts.zero_eq},
@@ -1587,15 +1588,15 @@ begin
 end,
 h f ([])
 
-def bounded_formula.rec {C : Πn, bounded_formula n → Sort v}
+def bounded_formula.rec {C : Πn, bounded_formula L n → Sort v}
   (hfalsum : Π {n}, C n ⊥)
-  (hequal : Π {n} (t₁ t₂ : bounded_term n), C n (t₁ ≃ t₂))
-  (hrel : Π {n l : ℕ} (R : L.relations l) (ts : dvector (bounded_term n) l), 
+  (hequal : Π {n} (t₁ t₂ : bounded_term L n), C n (t₁ ≃ t₂))
+  (hrel : Π {n l : ℕ} (R : L.relations l) (ts : dvector (bounded_term L n) l), 
     C n (bd_apps_rel (bd_rel R) ts))
-  (himp : Π {n} {f₁ f₂ : bounded_formula n} (ih₁ : C n f₁) (ih₂ : C n f₂), C n (f₁ ⟹ f₂))
-  (hall : Π {n} {f : bounded_formula (n+1)} (ih : C (n+1) f), C n (∀' f)) 
-  {{n : ℕ}} (f : bounded_formula n) : C n f :=
-have h : ∀{n l} (f : bounded_preformula n l) (ts : dvector (bounded_term n) l), 
+  (himp : Π {n} {f₁ f₂ : bounded_formula L n} (ih₁ : C n f₁) (ih₂ : C n f₂), C n (f₁ ⟹ f₂))
+  (hall : Π {n} {f : bounded_formula L (n+1)} (ih : C (n+1) f), C n (∀' f)) 
+  {{n : ℕ}} (f : bounded_formula L n) : C n f :=
+have h : ∀{n l} (f : bounded_preformula L n l) (ts : dvector (bounded_term L n) l), 
   C n (bd_apps_rel f ts),
 begin
   refine bounded_preformula.rec _ _ _ _ _ _; intros; try {rw ts.zero_eq},
@@ -1605,65 +1606,65 @@ end,
 h f ([])
 
 
-def lift_bounded_formula_at {n' l} (f : bounded_preformula n' l) (n m : ℕ) : 
-  bounded_preformula (n'+n) l :=
+def lift_bounded_formula_at {n' l} (f : bounded_preformula L n' l) (n m : ℕ) : 
+  bounded_preformula L (n'+n) l :=
 ⟨f.fst ↑' n # m, formula_below_lift n m f.snd⟩
 notation t ` ↑' `:90 n ` # `:90 m:90 := _root_.fol.lift_bounded_formula_at t n m -- input ↑ with \u or \upa
 
-@[reducible] def lift_bounded_formula {n' l} (f : bounded_preformula n' l) (n : ℕ) : 
-  bounded_preformula (n'+n) l := 
+@[reducible] def lift_bounded_formula {n' l} (f : bounded_preformula L n' l) (n : ℕ) : 
+  bounded_preformula L (n'+n) l := 
 f ↑' n # 0
 infix ` ↑ `:100 := _root_.fol.lift_bounded_formula -- input ↑' with \u or \upa
-@[reducible, simp] def lift_bounded_formula1 {n' l} (f : bounded_preformula n' l) : 
-  bounded_preformula (n'+1) l := 
+@[reducible, simp] def lift_bounded_formula1 {n' l} (f : bounded_preformula L n' l) : 
+  bounded_preformula L (n'+1) l := 
 f ↑ 1
 
-def substmax_bounded_formula {n l} (f : bounded_preformula (n+1) l) (t : closed_term) :
-  bounded_preformula n l :=
+def substmax_bounded_formula {n l} (f : bounded_preformula L (n+1) l) (t : closed_term L) :
+  bounded_preformula L n l :=
 ⟨f.fst[t.fst // n], formula_below_subst_closed f.snd t.snd⟩
 --notation f `[`:95 t ` // `:95 n `]`:0 := @_root_.fol.substmax_bounded_formula _ n _ f t
 
-lemma substmax_bounded_formula_bd_apps_rel {n l} (f : bounded_preformula (n+1) l) 
-  (t : closed_term) (ts : dvector (bounded_term (n+1)) l) :
+lemma substmax_bounded_formula_bd_apps_rel {n l} (f : bounded_preformula L (n+1) l) 
+  (t : closed_term L) (ts : dvector (bounded_term L (n+1)) l) :
   substmax_bounded_formula (bd_apps_rel f ts) t = 
   bd_apps_rel (substmax_bounded_formula f t) (ts.map $ λt', substmax_bounded_term t' t) :=
 begin
   induction ts generalizing f, refl, apply ts_ih (bd_apprel f ts_x)
 end
 
-def subst0_bounded_formula {n l} (f : bounded_preformula (n+1) l) (t : bounded_term n) :
-  bounded_preformula n l :=
+def subst0_bounded_formula {n l} (f : bounded_preformula L (n+1) l) (t : bounded_term L n) :
+  bounded_preformula L n l :=
 ⟨f.fst[t.fst // 0], formula_below_subst0 f.snd t.snd⟩
 
 notation f `[`:max s ` /0]`:0 := _root_.fol.subst0_bounded_formula f s
 
-@[simp] def substmax_eq_subst0 {l} (f : bounded_preformula 1 l) (t : closed_term) :
+@[simp] def substmax_eq_subst0 {l} (f : bounded_preformula L 1 l) (t : closed_term L) :
   f[t/0] = substmax_bounded_formula f t :=
 by refl
 
-def subst0_closed_formula {n l} (f : bounded_preformula (n+1) l) (t : closed_term) :
-  bounded_preformula n l :=
+def subst0_closed_formula {n l} (f : bounded_preformula L (n+1) l) (t : closed_term L) :
+  bounded_preformula L n l :=
 f [bounded_term_of_closed_term t/0]
 
-@[simp] def lift_presentence {l} (n m : ℕ) (f : presentence l) : f.fst ↑' n # m = f.fst :=
+@[simp] def lift_presentence {l} (n m : ℕ) (f : presentence L l) : f.fst ↑' n # m = f.fst :=
 lift_formula_below f.snd n m.zero_le
-@[simp] def lift_sentence (n m : ℕ) (f : sentence) : f.fst ↑' n # m = f.fst :=
+@[simp] def lift_sentence (n m : ℕ) (f : sentence L) : f.fst ↑' n # m = f.fst :=
 lift_presentence n m f
-@[simp] def lift_sentence1 (f : sentence) : f.fst ↑ 1 = f.fst :=
+@[simp] def lift_sentence1 (f : sentence L) : f.fst ↑ 1 = f.fst :=
 lift_presentence 1 0 f
 
-def realize_bounded_formula {S : Structure} {n} (v : dvector S n)
-  {l} (f : bounded_preformula n l) (xs : dvector S l) : Prop :=
+def realize_bounded_formula {S : Structure L} {n} (v : dvector S n)
+  {l} (f : bounded_preformula L n l) (xs : dvector S l) : Prop :=
 realize_formula_below v f.snd xs
 
-@[reducible] def realize_sentence (S : Structure) (f : sentence) : Prop :=
+@[reducible] def realize_sentence (S : Structure L) (f : sentence L) : Prop :=
 realize_bounded_formula ([] : dvector S 0) f ([])
 
 infix ` ⊨ `:51 := _root_.fol.realize_sentence -- input using \|= or \vDash, but not using \models 
 
 /- this is similar to realize_formula_below -/
 -- @[simp] def subst_formula_below : ∀ {n n' l} 
---   {f : preformula l} (hf : formula_below n f), arity (bounded_term n') (bounded_preformula n' l) n
+--   {f : preformula L l} (hf : formula_below n f), arity (bounded_term n') (bounded_preformula n' l) n
 -- | n n' _ _ b_falsum                 := arity_constant ⊥
 -- | n n' _ _ (b_equal' t₁ t₂ ht₁ ht₂) := sorry
 -- | n n' _ _ (b_rel R)                := arity_constant $ bd_rel R
@@ -1674,7 +1675,7 @@ infix ` ⊨ `:51 := _root_.fol.realize_sentence -- input using \|= or \vDash, bu
 --   arity_postcompose bd_all (arity_precompose (subst_formula_below hf &0) lift_bounded_term1)
 
 -- @[simp] def substitute_formula_below : ∀ {n n'} (v : dvector (bounded_term n') n) {l} 
---   {f : preformula l} (hf : formula_below n f), bounded_preformula n' l
+--   {f : preformula L l} (hf : formula_below n f), bounded_preformula L n' l
 -- | n n' v _ _ b_falsum                 := ⊥
 -- | n n' v _ _ (b_equal' t₁ t₂ ht₁ ht₂) := substitute_term_below v ht₁ ≃ substitute_term_below v ht₂
 -- | n n' v _ _ (b_rel R)                := bd_rel R
@@ -1685,11 +1686,11 @@ infix ` ⊨ `:51 := _root_.fol.realize_sentence -- input using \|= or \vDash, bu
 -- | n n' v _ _ (b_all' f hf)            := 
 --   ∀' substitute_formula_below (&0::v.map lift_bounded_term1) hf
 
--- @[simp] def substitute_bounded_formula {n n' l} (f : bounded_preformula n l) 
---   (v : dvector (bounded_term n') n) : bounded_preformula n' l :=
+-- @[simp] def substitute_bounded_formula {n n' l} (f : bounded_preformula L n l) 
+--   (v : dvector (bounded_term n') n) : bounded_preformula L n' l :=
 -- substitute_formula_below v f.snd
 
--- @[simp] def substitute_bounded_formula : ∀{n} (n') {l} (f : bounded_preformula n l), 
+-- @[simp] def substitute_bounded_formula : ∀{n} (n') {l} (f : bounded_preformula L n l), 
 --   arity (bounded_term n') (bounded_preformula n' l) n
 -- | 0     n' l f := ⟨f.fst, sorry⟩
 -- | (n+1) n' l f := λt, 
@@ -1697,29 +1698,29 @@ infix ` ⊨ `:51 := _root_.fol.realize_sentence -- input using \|= or \vDash, bu
 
   -- λt, arity_postcompose (λf, subst0_bounded_formula f t) (arity_precompose (substitute_bounded_formula (n'+1) _) lift_bounded_term1)
 
--- @[simp] def substitute_bounded_formula_arity : ∀{n l} (f : bounded_preformula n l), 
---   arity closed_term (presentence l) n
+-- @[simp] def substitute_bounded_formula_arity : ∀{n l} (f : bounded_preformula L n l), 
+--   arity closed_term L (presentence l) n
 -- | 0     l f := f
 -- | (n+1) l f := λt, substitute_bounded_formula_arity $ subst0_closed_formula f t
 
--- @[simp] def substitute_bounded_formula_arity_congr : ∀{n l} {f f' : bounded_preformula n l}
+-- @[simp] def substitute_bounded_formula_arity_congr : ∀{n l} {f f' : bounded_preformula L n l}
 --   (h : f.fst = f'.fst), substitute_bounded_formula_arity f = substitute_bounded_formula_arity f'
 -- | 0     l f f' h := sentence.eq h
 -- | (n+1) l f f' h := funext $ λt, substitute_bounded_formula_arity_congr $ 
 --   by dsimp [subst0_closed_formula, subst0_bounded_formula]; rw [h]
 
--- def substitute_bounded_formula {n l} (f : bounded_preformula n l) 
---   (v : dvector closed_term n) : presentence l :=
+-- def substitute_bounded_formula {n l} (f : bounded_preformula L n l) 
+--   (v : dvector (closed_term L) n) : presentence L l :=
 -- arity_app (substitute_bounded_formula_arity f) v
 
--- @[simp] def substitute_bounded_formula_congr {n l} {f f' : bounded_preformula n l}
---   (h : f.fst = f'.fst) (v : dvector closed_term n) : 
+-- @[simp] def substitute_bounded_formula_congr {n l} {f f' : bounded_preformula L n l}
+--   (h : f.fst = f'.fst) (v : dvector (closed_term L) n) : 
 --   substitute_bounded_formula f v = substitute_bounded_formula f' v :=
 -- by unfold substitute_bounded_formula; rw [substitute_bounded_formula_arity_congr h]
 
--- lemma substitute_bounded_formula_zero' {n l} (f : bounded_preformula n l) 
---   (v : dvector closed_term n) (h : 0 = n) : 
---   (cast (@congr_arg _ _ _ _ (λn, bounded_preformula n l) h.symm) f).fst = 
+-- lemma substitute_bounded_formula_zero' {n l} (f : bounded_preformula L n l) 
+--   (v : dvector (closed_term L) n) (h : 0 = n) : 
+--   (cast (@congr_arg _ _ _ _ (λn, bounded_preformula L n l) h.symm) f).fst = 
 --   (substitute_bounded_formula f v).fst :=
 -- begin
 --   induction f with f hf, induction hf; try { induction h },
@@ -1731,20 +1732,20 @@ infix ` ⊨ `:51 := _root_.fol.realize_sentence -- input using \|= or \vDash, bu
 --   simp [cast], congr1, sorry
 -- end
 
--- @[simp] lemma substitute_bounded_formula_zero {l} (f : presentence l) 
---   (v : dvector closed_term 0) : substitute_bounded_formula f v = f :=
+-- @[simp] lemma substitute_bounded_formula_zero {l} (f : presentence L l) 
+--   (v : dvector (closed_term L) 0) : substitute_bounded_formula f v = f :=
 -- sentence.eq (substitute_bounded_formula_zero' f v rfl).symm
 
--- @[simp] lemma substitute_bounded_formula_falsum {n} (v : dvector closed_term n) :
---   substitute_bounded_formula (⊥ : bounded_formula n) v = ⊥ :=
+-- @[simp] lemma substitute_bounded_formula_falsum {n} (v : dvector (closed_term L) n) :
+--   substitute_bounded_formula (⊥ : bounded_formula L n) v = ⊥ :=
 -- begin
 --   induction v,
 --   { simp },
 --   { refine eq.trans _ v_ih, refine substitute_bounded_formula_congr _ v_a_1, refl }
 -- end
 
--- @[simp] lemma substitute_bounded_formula_imp {n} (f₁ f₂ : bounded_formula n) 
---   (v : dvector closed_term n) : substitute_bounded_formula (f₁ ⟹ f₂) v = 
+-- @[simp] lemma substitute_bounded_formula_imp {n} (f₁ f₂ : bounded_formula L n) 
+--   (v : dvector (closed_term L) n) : substitute_bounded_formula (f₁ ⟹ f₂) v = 
 --   substitute_bounded_formula f₁ v ⟹ substitute_bounded_formula f₂ v :=
 -- begin
 --   induction v,
@@ -1755,8 +1756,8 @@ infix ` ⊨ `:51 := _root_.fol.realize_sentence -- input using \|= or \vDash, bu
 --     apply v_ih }
 -- end
 
--- @[simp] lemma substitute_bounded_formula_all {n} (f : bounded_formula (n+1)) 
---   (v : dvector closed_term n) : substitute_bounded_formula (∀' f) v = 
+-- @[simp] lemma substitute_bounded_formula_all {n} (f : bounded_formula L (n+1)) 
+--   (v : dvector (closed_term L) n) : substitute_bounded_formula (∀' f) v = 
 --   ∀' _ :=
 -- begin
 --   induction v,
@@ -1767,14 +1768,14 @@ infix ` ⊨ `:51 := _root_.fol.realize_sentence -- input using \|= or \vDash, bu
 --     apply v_ih }
 -- end
 
-@[simp] lemma realize_sentence_false {S : Structure} : S ⊨ (⊥ : sentence) ↔ false :=
+@[simp] lemma realize_sentence_false {S : Structure L} : S ⊨ (⊥ : sentence L) ↔ false :=
 by refl
-@[simp] lemma realize_sentence_imp {S : Structure} {f₁ f₂ : sentence} : 
+@[simp] lemma realize_sentence_imp {S : Structure L} {f₁ f₂ : sentence L} : 
   S ⊨ f₁ ⟹ f₂ ↔ (S ⊨ f₁ → S ⊨ f₂) :=
 by refl
-@[simp] lemma realize_sentence_not {S : Structure} {f : sentence} : S ⊨ ∼f ↔ ¬ S ⊨ f :=
+@[simp] lemma realize_sentence_not {S : Structure L} {f : sentence L} : S ⊨ ∼f ↔ ¬ S ⊨ f :=
 by refl
-@[simp] lemma realize_sentence_and {S : Structure} {f₁ f₂ : sentence} :
+@[simp] lemma realize_sentence_and {S : Structure L} {f₁ f₂ : sentence L} :
   S ⊨ f₁ ⊓ f₂ ↔ (S ⊨ f₁ ∧ S ⊨ f₂) :=
 begin
   have : S ⊨ f₁ ∧ S ⊨ f₂ ↔ ¬(S ⊨ f₁ → ¬ S ⊨ f₂),
@@ -1783,89 +1784,89 @@ begin
       {intro H, have := @not.elim _ (S ⊨ f₁) H, finish},
   rw[this], refl
 end
-@[simp] lemma realize_sentence_all {S : Structure} {f : bounded_formula 1} :
+@[simp] lemma realize_sentence_all {S : Structure L} {f : bounded_formula L 1} :
   (S ⊨ ∀'f) ↔ ∀ x : S, realize_bounded_formula([x]) f([]) :=
 by refl
 
-lemma realize_bounded_formula_bd_apps_rel {S : Structure}
-  {n l} (xs : dvector S n) (f : bounded_preformula n l) (ts : dvector (bounded_term n) l) :
+lemma realize_bounded_formula_bd_apps_rel {S : Structure L}
+  {n l} (xs : dvector S n) (f : bounded_preformula L n l) (ts : dvector (bounded_term L n) l) :
   realize_bounded_formula xs (bd_apps_rel f ts) ([]) ↔ 
   realize_bounded_formula xs f (ts.map (λt, realize_bounded_term xs t ([]))) :=
 begin
   induction ts generalizing f, refl, apply ts_ih (bd_apprel f ts_x)
 end
 
--- lemma realize_sentence_bd_apps_rel' {S : Structure}
---   {l} (f : presentence l) (ts : dvector closed_term l) :
+-- lemma realize_sentence_bd_apps_rel' {S : Structure L}
+--   {l} (f : presentence L l) (ts : dvector (closed_term L) l) :
 --   S ⊨ bd_apps_rel f ts ↔ realize_bounded_formula ([]) f (ts.map $ realize_closed_term S) :=
 -- realize_bounded_formula_bd_apps_rel ([]) f ts
 
-lemma realize_bd_apps_rel {S : Structure}
-  {l} (R : L.relations l) (ts : dvector closed_term l) :
+lemma realize_bd_apps_rel {S : Structure L}
+  {l} (R : L.relations l) (ts : dvector (closed_term L) l) :
   S ⊨ bd_apps_rel (s_rel R) ts ↔ S.rel_map R (ts.map $ realize_closed_term S) :=
 by apply realize_bounded_formula_bd_apps_rel ([]) (bd_rel R) ts
 
-lemma realize_sentence_equal {S : Structure} (t₁ t₂ : closed_term) :
+lemma realize_sentence_equal {S : Structure L} (t₁ t₂ : closed_term L) :
   S ⊨ t₁ ≃ t₂ ↔ realize_closed_term S t₁ = realize_closed_term S t₂  :=
 by refl
 
--- lemma realize_sentence_eq {S : Structure} (v : ℕ → S) (f : sentence) : 
+-- lemma realize_sentence_eq {S : Structure L} (v : ℕ → S) (f : sentence L) : 
 --   realize_sentence S f ↔ realize_formula v f.fst ([]) :=
 -- realize_formula_below_eq (λk hk, by exfalso; exact not_lt_zero k hk) f.snd _
 
-lemma realize_sentence_iff {S : Structure} (v : ℕ → S) (f : sentence) : 
+lemma realize_sentence_iff {S : Structure L} (v : ℕ → S) (f : sentence L) : 
   realize_sentence S f ↔ realize_formula v f.fst ([]) :=
 realize_formula_below_eq (λk hk, by exfalso; exact not_lt_zero k hk) f.snd _
 
-lemma realize_sentence_of_satisfied_in {S : Structure} [HS : nonempty S] {f : sentence} 
+lemma realize_sentence_of_satisfied_in {S : Structure L} [HS : nonempty S] {f : sentence L} 
   (H : S ⊨ f.fst) : S ⊨ f :=
 begin unfreezeI, induction HS with x, exact (realize_sentence_iff (λn, x) f).mpr (H _) end
 
-lemma satisfied_in_of_realize_sentence {S : Structure} {f : sentence} (H : S ⊨ f) : S ⊨ f.fst :=
+lemma satisfied_in_of_realize_sentence {S : Structure L} {f : sentence L} (H : S ⊨ f) : S ⊨ f.fst :=
 λv, (realize_sentence_iff v f).mp H
 
-lemma realize_sentence_iff_satisfied_in {S : Structure} [HS : nonempty S] {f : sentence} :
+lemma realize_sentence_iff_satisfied_in {S : Structure L} [HS : nonempty S] {f : sentence L} :
   S ⊨ f ↔ S ⊨ f.fst  :=
 ⟨satisfied_in_of_realize_sentence, realize_sentence_of_satisfied_in⟩
 
 /- theories -/
 
-parameter (L)
-@[reducible] def Theory := set sentence
-parameter {L}
+variable (L)
+@[reducible] def Theory := set $ sentence L
+variable {L}
 
-@[reducible] def Theory.fst (T : Theory) : set formula := sigma.fst '' T
+@[reducible] def Theory.fst (T : Theory L) : set (formula L) := sigma.fst '' T
 
-def sprf (T : Theory) (f : sentence) := T.fst ⊢ f.fst
+def sprf (T : Theory L) (f : sentence L) := T.fst ⊢ f.fst
 infix ` ⊢ `:51 := _root_.fol.sprf -- input: \|- or \vdash
 
-def sprovable (T : Theory) (f : sentence) := T.fst ⊢' f.fst
+def sprovable (T : Theory L) (f : sentence L) := T.fst ⊢' f.fst
 infix ` ⊢' `:51 := _root_.fol.sprovable -- input: \|- or \vdash
 
-def saxm {T : Theory} {A : sentence} (H : A ∈ T) : T ⊢ A := 
+def saxm {T : Theory L} {A : sentence L} (H : A ∈ T) : T ⊢ A := 
 by apply axm; apply mem_image_of_mem _ H
 
-def simpI {T : Theory} {A B : sentence} (H : insert A T ⊢ B) : T ⊢ A ⟹ B := 
+def simpI {T : Theory L} {A B : sentence L} (H : insert A T ⊢ B) : T ⊢ A ⟹ B := 
 begin
   apply impI, simp[sprf, Theory.fst, image_insert_eq] at H, assumption
 end
 
-@[reducible] lemma fst_commutes_with_imp {T : Theory} (A B : sentence) : (A ⟹ B).fst = A.fst ⟹ B.fst := by refl
+@[reducible] lemma fst_commutes_with_imp {T : Theory L} (A B : sentence L) : (A ⟹ B).fst = A.fst ⟹ B.fst := by refl
 
-def sfalsumE {T : Theory} {A : sentence} (H : insert ∼A T ⊢ s_falsum) : T ⊢ A :=
+def sfalsumE {T : Theory L} {A : sentence L} (H : insert ∼A T ⊢ s_falsum) : T ⊢ A :=
 begin
   apply falsumE, simp[sprf, Theory.fst, image_insert_eq] at H, assumption
 end
 
-def snotI {T : Theory} {A : sentence} (H : T ⊢ A ⟹ s_falsum) : T ⊢ (s_not A) :=
+def snotI {T : Theory L} {A : sentence L} (H : T ⊢ A ⟹ s_falsum) : T ⊢ (s_not A) :=
 begin
   apply notI, simp[sprf, Theory.fst, image_insert_eq] at H, assumption
 end
 
-def sandI {T : Theory} {A B : sentence} (H1 : T ⊢ A) (H2 : T ⊢ B) : T ⊢ A ⊓ B :=
+def sandI {T : Theory L} {A B : sentence L} (H1 : T ⊢ A) (H2 : T ⊢ B) : T ⊢ A ⊓ B :=
 andI H1 H2
 
-def snot_and_self {T : Theory} {A : sentence} (H : T ⊢ A ⊓ ∼ A) : T ⊢ s_falsum :=
+def snot_and_self {T : Theory L} {A : sentence L} (H : T ⊢ A ⊓ ∼ A) : T ⊢ s_falsum :=
 begin
 cases A with A and hA,
 fapply not_and_self,
@@ -1873,89 +1874,89 @@ exact A, simp[sprf] at H,
 exact H
 end
 
-def sprovable_of_provable {T : Theory} {f : sentence} (h : T.fst ⊢ f.fst) : T ⊢ f := h
-def provable_of_sprovable {T : Theory} {f : sentence} (h : T ⊢ f) : T.fst ⊢ f.fst := h
+def sprovable_of_provable {T : Theory L} {f : sentence L} (h : T.fst ⊢ f.fst) : T ⊢ f := h
+def provable_of_sprovable {T : Theory L} {f : sentence L} (h : T ⊢ f) : T.fst ⊢ f.fst := h
 
--- def sprovable_of_sprovable_lift_at {T : Theory} (n m : ℕ) {f : formula} (h : T.fst ⊢ f ↑' n # m) :
+-- def sprovable_of_sprovable_lift_at {T : Theory L} (n m : ℕ) {f : formula L} (h : T.fst ⊢ f ↑' n # m) :
 --   T.fst ⊢ f := 
 -- sorry
 
--- def sprovable_of_sprovable_lift {T : Theory} {f : formula} (h : T.fst ⊢ f ↑ 1) : T.fst ⊢ f := 
+-- def sprovable_of_sprovable_lift {T : Theory L} {f : formula L} (h : T.fst ⊢ f ↑ 1) : T.fst ⊢ f := 
 -- sprovable_of_sprovable_lift_at 1 0 h
 
-def sprovable_lift {T : Theory} {f : formula} (h : T.fst ⊢ f) : T.fst ⊢ f ↑ 1 := 
+def sprovable_lift {T : Theory L} {f : formula L} (h : T.fst ⊢ f) : T.fst ⊢ f ↑ 1 := 
 begin
   have := prf_lift 1 0 h, dsimp [Theory.fst] at this, 
   rw [←image_comp, image_congr' lift_sentence1] at this, exact this
 end
 
-def all_sprovable (T T' : Theory) := ∀(f ∈ T'), T ⊢ f
+def all_sprovable (T T' : Theory L) := ∀(f ∈ T'), T ⊢ f
 infix ` ⊢ `:51 := _root_.fol.all_sprovable -- input: \|- or \vdash
 
-def all_realize_sentence (S : Structure) (T : Theory) := ∀{{f}}, f ∈ T → S ⊨ f
+def all_realize_sentence (S : Structure L) (T : Theory L) := ∀{{f}}, f ∈ T → S ⊨ f
 infix ` ⊨ `:51 := _root_.fol.all_realize_sentence -- input using \|= or \vDash, but not using \models 
 
-def ssatisfied (T : Theory) (f : sentence) := 
-∀{{S : Structure}}, nonempty S → S ⊨ T → S ⊨ f
+def ssatisfied (T : Theory L) (f : sentence L) := 
+∀{{S : Structure L}}, nonempty S → S ⊨ T → S ⊨ f
 
 infix ` ⊨ `:51 := _root_.fol.ssatisfied -- input using \|= or \vDash, but not using \models 
 
-def all_ssatisfied (T T' : Theory) := ∀(f ∈ T'), T ⊨ f
+def all_ssatisfied (T T' : Theory L) := ∀(f ∈ T'), T ⊨ f
 infix ` ⊨ `:51 := _root_.fol.all_ssatisfied -- input using \|= or \vDash, but not using \models 
 
-def satisfied_of_ssatisfied {T : Theory} {f : sentence} (H : T ⊨ f) : T.fst ⊨ f.fst :=
+def satisfied_of_ssatisfied {T : Theory L} {f : sentence L} (H : T ⊨ f) : T.fst ⊨ f.fst :=
 begin
   intros S v hT, rw [←realize_sentence_iff], apply H ⟨ v 0 ⟩,
   intros f' hf', rw [realize_sentence_iff v], apply hT, apply mem_image_of_mem _ hf'
 end
 
-def ssatisfied_of_satisfied {T : Theory} {f : sentence} (H : T.fst ⊨ f.fst) : T ⊨ f :=
+def ssatisfied_of_satisfied {T : Theory L} {f : sentence L} (H : T.fst ⊨ f.fst) : T ⊨ f :=
 begin
   intros S hS hT, induction hS with s, rw [realize_sentence_iff (λ_, s)], apply H,
   intros f' hf', rcases hf' with ⟨f', ⟨hf', h⟩⟩, induction h, rw [←realize_sentence_iff],
   exact hT hf'
 end
 
-def all_satisfied_of_all_ssatisfied {T T' : Theory} (H : T ⊨ T') : T.fst ⊨ T'.fst :=
+def all_satisfied_of_all_ssatisfied {T T' : Theory L} (H : T ⊨ T') : T.fst ⊨ T'.fst :=
 begin intros f hf, rcases hf with ⟨f, ⟨hf, rfl⟩⟩, apply satisfied_of_ssatisfied (H f hf) end
 
-def all_ssatisfied_of_all_satisfied {T T' : Theory} (H : T.fst ⊨ T'.fst) : T ⊨ T' :=
+def all_ssatisfied_of_all_satisfied {T T' : Theory L} (H : T.fst ⊨ T'.fst) : T ⊨ T' :=
 begin intros f hf, apply ssatisfied_of_satisfied, apply H, exact mem_image_of_mem _ hf end
 
-def satisfied_iff_ssatisfied {T : Theory} {f : sentence} : T ⊨ f ↔ T.fst ⊨ f.fst :=
+def satisfied_iff_ssatisfied {T : Theory L} {f : sentence L} : T ⊨ f ↔ T.fst ⊨ f.fst :=
 ⟨satisfied_of_ssatisfied, ssatisfied_of_satisfied⟩
 
-def all_satisfied_sentences_iff {T T' : Theory} : T ⊨ T' ↔ T.fst ⊨ T'.fst :=
+def all_satisfied_sentences_iff {T T' : Theory L} : T ⊨ T' ↔ T.fst ⊨ T'.fst :=
 ⟨all_satisfied_of_all_ssatisfied, all_ssatisfied_of_all_satisfied⟩
 
-def ssatisfied_snot {S : Structure} {f : sentence} (hS : ¬(S ⊨ f)) : S ⊨ ∼ f := 
+def ssatisfied_snot {S : Structure L} {f : sentence L} (hS : ¬(S ⊨ f)) : S ⊨ ∼ f := 
 by exact hS
 
-def Model (T : Theory) : Type (u+1) := Σ' (S : Structure), S ⊨ T
+def Model (T : Theory L) : Type (u+1) := Σ' (S : Structure L), S ⊨ T
 
-lemma soundness {T : Theory} {A : sentence} (H : T ⊢ A) : T ⊨ A :=
+lemma soundness {T : Theory L} {A : sentence L} (H : T ⊢ A) : T ⊨ A :=
 ssatisfied_of_satisfied $ formula_soundness H
 
-def is_consistent (T : Theory) := ¬(T ⊢' (⊥ : sentence))
+def is_consistent (T : Theory L) := ¬(T ⊢' (⊥ : sentence L))
 
-protected def is_consistent.intro {T : Theory} (H : ¬ T ⊢' (⊥ : sentence)) : is_consistent T :=
+protected def is_consistent.intro {T : Theory L} (H : ¬ T ⊢' (⊥ : sentence L)) : is_consistent T :=
 H
 
-protected def is_consistent.elim {T : Theory} (H : is_consistent T) : ¬ T ⊢' (⊥ : sentence)
+protected def is_consistent.elim {T : Theory L} (H : is_consistent T) : ¬ T ⊢' (⊥ : sentence L)
 | H' := H H'
 
-def is_complete (T : Theory) := 
-is_consistent T ∧ ∀(f : sentence), f ∈ T ∨ ∼ f ∈ T
+def is_complete (T : Theory L) := 
+is_consistent T ∧ ∀(f : sentence L), f ∈ T ∨ ∼ f ∈ T
 
-def mem_of_sprf {T : Theory} (H : is_complete T) {f : sentence} (Hf : T ⊢ f) : f ∈ T :=
+def mem_of_sprf {T : Theory L} (H : is_complete T) {f : sentence L} (Hf : T ⊢ f) : f ∈ T :=
 begin 
   cases H.2 f, exact h, exfalso, apply H.1, constructor, exact impE _ (saxm h) Hf, 
 end
 
-def mem_of_sprovable {T : Theory} (H : is_complete T) {f : sentence} (Hf : T ⊢' f) : f ∈ T :=
+def mem_of_sprovable {T : Theory L} (H : is_complete T) {f : sentence L} (Hf : T ⊢' f) : f ∈ T :=
 by destruct Hf; exact mem_of_sprf H
 
-def sprovable_of_sprovable_or {T : Theory} (H : is_complete T) {f₁ f₂ : sentence}
+def sprovable_of_sprovable_or {T : Theory L} (H : is_complete T) {f₁ f₂ : sentence L}
   (H₂ : T ⊢' f₁ ⊔ f₂) : (T ⊢' f₁) ∨ T ⊢' f₂ :=
 begin
   cases H.2 f₁ with h h, { left, exact ⟨saxm h⟩ },
@@ -1965,7 +1966,7 @@ begin
     [exact mem_image_of_mem _ h, exact mem_image_of_mem _ h']
 end
 
-def impI_of_is_complete {T : Theory} (H : is_complete T) {f₁ f₂ : sentence}
+def impI_of_is_complete {T : Theory L} (H : is_complete T) {f₁ f₂ : sentence L}
   (H₂ : T ⊢' f₁ → T ⊢' f₂) : T ⊢' f₁ ⟹ f₂ :=
 begin
   apply nonempty.map impI, cases H.2 f₁, 
@@ -1974,19 +1975,19 @@ begin
   apply nonempty.map2 (impE _) (nonempty.map weakening1 ⟨saxm h⟩) ⟨axm1⟩
 end
 
-def notI_of_is_complete {T : Theory} (H : is_complete T) {f : sentence}
+def notI_of_is_complete {T : Theory L} (H : is_complete T) {f : sentence L}
   (H₂ : ¬T ⊢' f) : T ⊢' ∼f :=
 begin
   apply @impI_of_is_complete _ T H f s_falsum,
   intro h, exfalso, exact H₂ h
 end
 
-def has_enough_constants (T : Theory) :=
-∃(C : Π(f : bounded_formula 1), L.constants), 
-∀(f : bounded_formula 1), T ⊢' ∃' f ⟹ f[c_const (C f)/0]
+def has_enough_constants (T : Theory L) :=
+∃(C : Π(f : bounded_formula L 1), L.constants), 
+∀(f : bounded_formula L 1), T ⊢' ∃' f ⟹ f[c_const (C f)/0]
 
-def find_counterexample_of_henkin {T : Theory} (H₁ : is_complete T) (H₂ : has_enough_constants T) 
-  (f : bounded_formula 1) (H₃ : ¬ T ⊢' ∀' f) : ∃(t : closed_term), T ⊢' ∼ f[t/0] :=
+def find_counterexample_of_henkin {T : Theory L} (H₁ : is_complete T) (H₂ : has_enough_constants T) 
+  (f : bounded_formula L 1) (H₃ : ¬ T ⊢' ∀' f) : ∃(t : closed_term L), T ⊢' ∼ f[t/0] :=
 begin
   induction H₂ with C HC, 
   refine ⟨c_const (C (∼ f)), _⟩,
@@ -1995,37 +1996,39 @@ begin
 end
 
 section completeness
-parameters {T : Theory} (H₁ : is_complete T) (H₂ : has_enough_constants T)
-def term_rel (t₁ t₂ : closed_term) : Prop := T ⊢' t₁ ≃ t₂
+variables (T : Theory L) (H₁ : is_complete T) (H₂ : has_enough_constants T)
+def term_rel (t₁ t₂ : closed_term L) : Prop := T ⊢' t₁ ≃ t₂
 
-def term_setoid : setoid closed_term := 
-⟨term_rel, λt, ⟨refl _ _⟩, λt t' H, H.map symm, λt₁ t₂ t₃ H₁ H₂, H₁.map2 trans H₂⟩
+def term_setoid : setoid $ closed_term L := 
+⟨term_rel T, λt, ⟨ref _ _⟩, λt t' H, H.map symm, λt₁ t₂ t₃ H₁ H₂, H₁.map2 trans H₂⟩
 local attribute [instance] term_setoid
 
 def term_model' : Type u :=
-quotient term_setoid
+quotient $ term_setoid T
 -- set_option pp.all true
 -- #print term_setoid
 -- set_option trace.class_instances true
 
-def term_model_fun' {l} (t : closed_preterm l) (ts : dvector closed_term l) : term_model' :=
-@quotient.mk _ term_setoid $ c_apps t ts
+def term_model_fun' {l} (t : closed_preterm L l) (ts : dvector (closed_term L) l) : term_model' T :=
+@quotient.mk _ (term_setoid T) $ c_apps t ts
 
--- def equal_preterms_trans {T : set formula} : ∀{l} {t₁ t₂ t₃ : preterm l} 
+-- def equal_preterms_trans {T : set (formula L)} : ∀{l} {t₁ t₂ t₃ : preterm L l} 
 --   (h₁₂ : equal_preterms T t₁ t₂) (h₂₃ : equal_preterms T t₂ t₃), equal_preterms T t₁ t₃ 
 
-def term_model_fun_eq {l} (t t' : closed_preterm (l+1)) (x x' : closed_term)
-  (Ht : equal_preterms T.fst t.fst t'.fst) (Hx : T ⊢ x ≃ x') (ts : dvector closed_term l) : 
-  term_model_fun' (c_app t x) ts = term_model_fun' (c_app t' x') ts :=
+variable {T}
+def term_model_fun_eq {l} (t t' : closed_preterm L (l+1)) (x x' : closed_term L)
+  (Ht : equal_preterms T.fst t.fst t'.fst) (Hx : T ⊢ x ≃ x') (ts : dvector (closed_term L) l) : 
+  term_model_fun' T (c_app t x) ts = term_model_fun' T (c_app t' x') ts :=
 begin
   induction ts generalizing x x',
   { apply quotient.sound, refine ⟨trans (app_congr t.fst Hx) _⟩, apply Ht ([x'.fst]) }, 
-  { apply ts_ih, apply equal_preterms_app Ht Hx, apply refl }
+  { apply ts_ih, apply equal_preterms_app Ht Hx, apply ref }
 end
 
-def term_model_fun {l} (t : closed_preterm l) (ts : dvector term_model' l) : term_model' :=
+variable (T)
+def term_model_fun {l} (t : closed_preterm L l) (ts : dvector (term_model' T) l) : term_model' T :=
 begin
-  refine ts.quotient_lift (term_model_fun' t) _, clear ts,
+  refine ts.quotient_lift (term_model_fun' T t) _, clear ts,
   intros ts ts' hts,
   induction hts,
   { refl },
@@ -2033,22 +2036,24 @@ begin
     refl, exact h }
 end
 
-def term_model_rel' {l} (f : presentence l) (ts : dvector closed_term l) : Prop :=
+def term_model_rel' {l} (f : presentence L l) (ts : dvector (closed_term L) l) : Prop :=
 T ⊢' s_apps_rel f ts
 
-def term_model_rel_iff {l} (f f' : presentence (l+1)) (x x' : closed_term)
-  (Ht : equiv_preformulae T.fst f.fst f'.fst) (Hx : T ⊢ x ≃ x') (ts : dvector closed_term l) : 
-  term_model_rel' (s_apprel f x) ts ↔ term_model_rel' (s_apprel f' x') ts :=
+variable {T}
+def term_model_rel_iff {l} (f f' : presentence L (l+1)) (x x' : closed_term L)
+  (Ht : equiv_preformulae T.fst f.fst f'.fst) (Hx : T ⊢ x ≃ x') (ts : dvector (closed_term L) l) : 
+  term_model_rel' T (s_apprel f x) ts ↔ term_model_rel' T (s_apprel f' x') ts :=
 begin
   induction ts generalizing x x',
   { apply iff.trans (apprel_congr' f.fst Hx), 
     apply iff_of_biimp, have := Ht ([x'.fst]), exact ⟨this⟩ }, 
-  { apply ts_ih, apply equiv_preformulae_apprel Ht Hx, apply refl }
+  { apply ts_ih, apply equiv_preformulae_apprel Ht Hx, apply ref }
 end
 
-def term_model_rel {l} (f : presentence l) (ts : dvector term_model' l) : Prop :=
+variable (T)
+def term_model_rel {l} (f : presentence L l) (ts : dvector (term_model' T) l) : Prop :=
 begin
-  refine ts.quotient_lift (term_model_rel' f) _, exact T, clear ts,
+  refine ts.quotient_lift (term_model_rel' T f) _, clear ts,
   intros ts ts' hts,
   induction hts,
   { refl },
@@ -2056,16 +2061,16 @@ begin
     refl, exact h }
 end
 
-def term_model : Structure :=
-⟨term_model', 
- λn, term_model_fun ∘ c_func, 
- λn, term_model_rel ∘ s_rel⟩
+def term_model : Structure L :=
+⟨term_model' T, 
+ λn, term_model_fun T ∘ c_func, 
+ λn, term_model_rel T ∘ s_rel⟩
 
-@[reducible] def term_mk : closed_term → term_model :=
-@quotient.mk _ term_setoid
+@[reducible] def term_mk : closed_term L → term_model T :=
+@quotient.mk _ $ term_setoid T
 
--- lemma realize_bounded_preterm_term_model {l n} (ts : dvector closed_term l) 
---   (t : bounded_preterm l n) (ts' : dvector closed_term n) :
+-- lemma realize_bounded_preterm_term_model {l n} (ts : dvector (closed_term L) l) 
+--   (t : bounded_preterm L l n) (ts' : dvector (closed_term L) n) :
 --   realize_bounded_term (ts.map term_mk) t (ts'.map term_mk) = 
 --   (term_mk _) :=
 -- begin
@@ -2076,8 +2081,9 @@ def term_model : Structure :=
 -- dsimp [term_model, Structure.rel_map, term_model_rel], 
 --     rw [ts.map_congr realize_closed_term_term_model, dvector.quotient_beta], refl
 
-lemma realize_closed_preterm_term_model {l} (ts : dvector closed_term l) (t : closed_preterm l) : 
-  realize_bounded_term ([]) t (ts.map term_mk) = (term_mk (bd_apps t ts)) :=
+variable {T}
+lemma realize_closed_preterm_term_model {l} (ts : dvector (closed_term L) l) (t : closed_preterm L l) : 
+  realize_bounded_term ([]) t (ts.map $ term_mk T) = (term_mk T (bd_apps t ts)) :=
 begin
   revert l t, refine bounded_preterm.rec _ _ _; intros,
   { apply k.fin_zero_elim },
@@ -2087,12 +2093,12 @@ begin
     apply ih_t (s::ts) }
 end
 
-@[simp] lemma realize_closed_term_term_model (t : closed_term) :
-  realize_closed_term term_model t = term_mk t :=
+@[simp] lemma realize_closed_term_term_model (t : closed_term L) :
+  realize_closed_term (term_model T) t = term_mk T t :=
 by apply realize_closed_preterm_term_model ([]) t
 
-lemma realize_subst_preterm {S : Structure} {n l} (t : bounded_preterm (n+1) l)
-  (xs : dvector S l) (s : closed_term) (v : dvector S n) :
+lemma realize_subst_preterm {S : Structure L} {n l} (t : bounded_preterm L (n+1) l)
+  (xs : dvector S l) (s : closed_term L) (v : dvector S n) :
   realize_bounded_term v (substmax_bounded_term t s) xs =
   realize_bounded_term (v.concat (realize_closed_term S s)) t xs :=
 begin
@@ -2114,14 +2120,14 @@ begin
     congr1, apply t_ih_s ([]) }
 end
 
-lemma realize_subst_term {S : Structure} {n} (v : dvector S n) (s : closed_term) 
-  (t : bounded_term (n+1))  :
+lemma realize_subst_term {S : Structure L} {n} (v : dvector S n) (s : closed_term L) 
+  (t : bounded_term L (n+1))  :
   realize_bounded_term v (substmax_bounded_term t s) ([]) =
   realize_bounded_term (v.concat (realize_closed_term S s)) t ([]) :=
 by apply realize_subst_preterm t ([]) s v
 
-lemma realize_subst_formula (S : Structure) {n} (f : bounded_formula (n+1))
-  (t : closed_term) (v : dvector S n) :
+lemma realize_subst_formula (S : Structure L) {n} (f : bounded_formula L (n+1))
+  (t : closed_term L) (v : dvector S n) :
   realize_bounded_formula v (substmax_bounded_formula f t) ([]) ↔
   realize_bounded_formula (v.concat (realize_closed_term S t)) f ([]) :=
 begin
@@ -2136,24 +2142,24 @@ begin
   { apply forall_congr, intro x, apply ih (x::v) }
 end
 
-lemma realize_subst_formula0 (S : Structure) (f : bounded_formula 1) (t : closed_term) :
+lemma realize_subst_formula0 (S : Structure L) (f : bounded_formula L 1) (t : closed_term L) :
   S ⊨ f[t/0] ↔ realize_bounded_formula ([realize_closed_term S t]) f ([]) :=
 by apply realize_subst_formula S f t ([])
 
-lemma term_model_subst0 (f : bounded_formula 1) (t : closed_term) :
-  term_model ⊨ f[t/0] ↔ realize_bounded_formula ([term_mk t]) f ([]) :=
-(realize_subst_formula0 term_model f t).trans (by simp)
+lemma term_model_subst0 (f : bounded_formula L 1) (t : closed_term L) :
+  term_model T ⊨ f[t/0] ↔ realize_bounded_formula ([term_mk T t]) f ([]) :=
+(realize_subst_formula0 (term_model T) f t).trans (by simp)
 
 include H₂
-instance nonempty_term_model : nonempty term_model :=
+instance nonempty_term_model : nonempty $ term_model T :=
 begin
-  induction H₂ with C, exact ⟨term_mk (c_const (C (&0 ≃ &0)))⟩
+  induction H₂ with C, exact ⟨term_mk T (c_const (C (&0 ≃ &0)))⟩
 end
 
 include H₁
-def term_model_ssatisfied_iff : ∀{n l} (f : presentence l) 
-  (ts : dvector closed_term l) (h : count_quantifiers f.fst < n),
-  T ⊢' s_apps_rel f ts ↔ term_model ⊨ s_apps_rel f ts :=
+def term_model_ssatisfied_iff : ∀{n l} (f : presentence L l) 
+  (ts : dvector (closed_term L) l) (h : count_quantifiers f.fst < n),
+  T ⊢' s_apps_rel f ts ↔ term_model T ⊨ s_apps_rel f ts :=
 begin
   intro n, refine nat.strong_induction_on n _, clear n,
   intros n n_ih l f ts hn,
@@ -2169,7 +2175,7 @@ begin
     have ih₂ := f_ih_f₂ ([]) hf_hf₂ (lt_of_le_of_lt (nat.le_add_left _ _) hn),
     split; intro h,
     { intro h₁, apply ih₂.mp, apply h.map2 (impE _), refine ih₁.mpr h₁ },
-    { change term_model ⊨ sigma.mk f_f₁ hf_hf₁ ⟹ sigma.mk f_f₂ hf_hf₂ at h,
+    { change term_model T ⊨ sigma.mk f_f₁ hf_hf₁ ⟹ sigma.mk f_f₂ hf_hf₂ at h,
       simp at h, simp at ih₁, rw [←ih₁] at h, simp at ih₂, rw [←ih₂] at h,
       exact impI_of_is_complete H₁ h }},
   { split; intro h,
@@ -2185,31 +2191,31 @@ begin
       cases n with n, { exfalso, exact not_lt_zero _ hn },
       refine (n_ih n (lt.base n) (⟨f_f, hf_hf⟩[t/0]) ([]) _).mpr _,
       { dsimp [subst0_bounded_formula], rw [count_quantifiers_subst], exact lt_of_succ_lt_succ hn },
-      exact (term_model_subst0 ⟨f_f, hf_hf⟩ t).mpr (h (term_mk t)) }},
+      exact (term_model_subst0 ⟨f_f, hf_hf⟩ t).mpr (h (term_mk T t)) }},
 end
 
-def term_model_ssatisfied : term_model ⊨ T :=
+def term_model_ssatisfied : term_model T ⊨ T :=
 begin
   intros f hf, apply (term_model_ssatisfied_iff H₁ H₂ f ([]) (lt.base _)).mp, exact ⟨saxm hf⟩
 end
 
 -- completeness for complete theories with enough constants
-lemma completeness' {f : sentence} (H : T ⊨ f) : T ⊢' f :=
+lemma completeness' {f : sentence L} (H : T ⊨ f) : T ⊢' f :=
 begin
   apply (term_model_ssatisfied_iff H₁ H₂ f ([]) (lt.base _)).mpr,
-  apply H, exact fol.nonempty_term_model, 
+  apply H, exact fol.nonempty_term_model H₂, 
   apply term_model_ssatisfied H₁ H₂,
 end
 
 end completeness
 
-def Th (S : Structure) : Theory := { f : sentence | S ⊨ f }
+def Th (S : Structure L) : Theory L := { f : sentence L | S ⊨ f }
 
-lemma realize_sentence_Th (S : Structure) : S ⊨ Th S :=
+lemma realize_sentence_Th (S : Structure L) : S ⊨ Th S :=
 λf hf, hf
 
-lemma is_complete_Th (S : Structure) (HS : nonempty S) : is_complete (Th S) :=
-⟨λH, by cases H; apply soundness H HS (realize_sentence_Th S), λ(f : sentence), classical.em (S ⊨ f)⟩
+lemma is_complete_Th (S : Structure L) (HS : nonempty S) : is_complete (Th S) :=
+⟨λH, by cases H; apply soundness H HS (realize_sentence_Th S), λ(f : sentence L), classical.em (S ⊨ f)⟩
 
 /- maybe define 
 presburger_arithmetic := Th (Z,+,0)
